zoo_parabs/vertex: Specification without ghost name.

theories/zoo_parabs/vertex.v
@@ -28,12 +28,6 @@ From zoo_parabs Require Import
 From zoo Require Import
   options.
 
-Implicit Types b finished : bool.
-Implicit Types preds : nat.
-Implicit Types t succ : location.
-Implicit Types task ctx : val.
-Implicit Types own : ownership.
-
 Inductive state :=
   | Init
   | Released
@@ -94,854 +88,1066 @@ Proof.
   solve_inG.
 Qed.
 
-Section vertex_G.
-  Context `{vertex_G : VertexG Σ}.
+Module raw.
+  Implicit Types b finished : bool.
+  Implicit Types preds : nat.
+  Implicit Types t succ : location.
+  Implicit Types task ctx : val.
+  Implicit Types own : ownership.
 
-  Implicit Types P Q R : iProp Σ.
+  Section vertex_G.
+    Context `{vertex_G : VertexG Σ}.
 
-  #[local] Definition state₁' γ_state own state :=
-    twins_twin1 (twins_G := vertex_G_state_G) γ_state own state.
-  #[local] Definition state₁ γ :=
-    state₁' γ.(vertex_name_state).
-  #[local] Definition state₂' γ_state state :=
-    twins_twin2 (twins_G := vertex_G_state_G) γ_state state.
-  #[local] Definition state₂ γ :=
-    state₂' γ.(vertex_name_state).
+    Implicit Types P Q R : iProp Σ.
 
-  #[local] Definition generation₁' γ_generation gen :=
-    twins_twin1 γ_generation (DfracOwn 1) gen.
-  #[local] Definition generation₁ γ :=
-    generation₁' γ.(vertex_name_generation).
-  #[local] Definition generation₂' γ_generation gen :=
-    twins_twin2 γ_generation gen.
-  #[local] Definition generation₂ γ :=
-    generation₂' γ.(vertex_name_generation).
+    #[local] Definition state₁' γ_state own state :=
+      twins_twin1 (twins_G := vertex_G_state_G) γ_state own state.
+    #[local] Definition state₁ γ :=
+      state₁' γ.(vertex_name_state).
+    #[local] Definition state₂' γ_state state :=
+      twins_twin2 (twins_G := vertex_G_state_G) γ_state state.
+    #[local] Definition state₂ γ :=
+      state₂' γ.(vertex_name_state).
 
-  #[local] Definition dependencies_auth gen own :=
-    mono_gmultiset_auth gen own.
-  #[local] Definition dependencies_elem gen :=
-    mono_gmultiset_elem gen.
+    #[local] Definition generation₁' γ_generation gen :=
+      twins_twin1 γ_generation (DfracOwn 1) gen.
+    #[local] Definition generation₁ γ :=
+      generation₁' γ.(vertex_name_generation).
+    #[local] Definition generation₂' γ_generation gen :=
+      twins_twin2 γ_generation gen.
+    #[local] Definition generation₂ γ :=
+      generation₂' γ.(vertex_name_generation).
 
-  #[local] Definition predecessors_auth' γ_predecessors Π :=
-    auth_gmultiset_auth γ_predecessors (DfracOwn 1) Π.
-  #[local] Definition predecessors_auth γ Π :=
-    predecessors_auth' γ.(vertex_name_predecessors) Π.
-  #[local] Definition predecessors_elem γ π :=
-    auth_gmultiset_frag γ.(vertex_name_predecessors) {[+π+]}.
+    #[local] Definition dependencies_auth gen own :=
+      mono_gmultiset_auth gen own.
+    #[local] Definition dependencies_elem gen :=
+      mono_gmultiset_elem gen.
 
-  #[local] Definition output_auth' γ_output :=
-    subprops_auth γ_output.
-  #[local] Definition output_auth γ :=
-    subprops_auth γ.(vertex_name_output).
-  #[local] Definition output_frag' γ_output :=
-    subprops_frag γ_output.
-  #[local] Definition output_frag γ :=
-    output_frag' γ.(vertex_name_output).
+    #[local] Definition predecessors_auth' γ_predecessors Π :=
+      auth_gmultiset_auth γ_predecessors (DfracOwn 1) Π.
+    #[local] Definition predecessors_auth γ Π :=
+      predecessors_auth' γ.(vertex_name_predecessors) Π.
+    #[local] Definition predecessors_elem γ π :=
+      auth_gmultiset_frag γ.(vertex_name_predecessors) {[+π+]}.
 
-  #[local] Definition model' t γ task state gen : iProp Σ :=
-    t.[task] ↦ task ∗
-    state₁ γ Own state ∗
-    generation₁ γ gen.
-  #[local] Instance : CustomIpatFormat "model'" :=
-    "(
-      Ht{which;}_task{_{}} &
-      Hstate{which;}₁{_{}} &
-      Hgeneration{which;}₁{_{}}
-    )".
-  Definition vertex_model t γ task gen : iProp Σ :=
-    model' t γ task Init gen.
-  #[local] Instance : CustomIpatFormat "model" :=
-    "(:model' {//} {/which/})".
+    #[local] Definition output_auth' γ_output :=
+      subprops_auth γ_output.
+    #[local] Definition output_auth γ :=
+      subprops_auth γ.(vertex_name_output).
+    #[local] Definition output_frag' γ_output :=
+      subprops_frag γ_output.
+    #[local] Definition output_frag γ :=
+      output_frag' γ.(vertex_name_output).
 
-  Definition vertex_running gen : iProp Σ :=
-    ∃ Δ,
-    dependencies_auth gen Discard Δ ∗
-    [∗ mset] δ ∈ Δ, state₁ δ Discard Finished.
-  #[local] Instance : CustomIpatFormat "running" :=
-    "(
-      %Δ{} &
-      #Hdependencies{which;}_auth{_{}} &
-      #HΔ{}
-    )".
-
-  Definition vertex_finished γ :=
-    state₁ γ Discard Finished.
-  #[local] Instance : CustomIpatFormat "finished" :=
-    "#Hstate{which;}₁{_{}}".
-
-  Definition vertex_wp_body t γ P R body task gen : iProp Σ :=
-    ∀ pool ctx gen',
-    pool_context pool ctx -∗
-    vertex_running gen -∗
-    vertex_model t γ task gen' -∗
-    WP task ctx {{ res,
-      ∃ b task,
-      ⌜res = #b⌝ ∗
-      ▷ (
-        pool_context pool ctx ∗
-        vertex_model t γ task gen' ∗
-        if b then
-          body task gen'
-        else
-          P ∗
-          □ R
-      )
-    }}.
-  #[local] Definition vertex_wp_pre
-  : location → vertex_name → iProp Σ → iProp Σ →
-    (val -d> vertex_generation -d> iProp Σ) →
-    val -d> vertex_generation -d> iProp Σ
-  :=
-    vertex_wp_body.
-  #[local] Instance vertex_wp_pre_contractive t γ P R :
-    Contractive (vertex_wp_pre t γ P R).
-  Proof.
-    rewrite /vertex_wp_pre /vertex_wp_body.
-    solve_contractive.
-  Qed.
-  #[local] Instance vertex_wp_pre_ne t γ P R :
-    NonExpansive (vertex_wp_pre t γ P R).
-  Proof.
-    apply _.
-  Qed.
-  Definition vertex_wp t γ P R : val → vertex_generation → iProp Σ :=
-    fixpoint (vertex_wp_pre t γ P R).
-
-  Lemma vertex_wp_unfold t γ P R task gen :
-    vertex_wp t γ P R task gen ⊣⊢
-    vertex_wp_body t γ P R (vertex_wp t γ P R) task gen.
-  Proof.
-    apply (fixpoint_unfold (vertex_wp_pre t γ P R)).
-  Qed.
-  #[global] Instance vertex_wp_ne n :
-    Proper (
-      (=) ==>
-      (=) ==>
-      (≡{n}≡) ==>
-      (≡{n}≡) ==>
-      (≡{n}≡) ==>
-      (≡{n}≡) ==>
-      (≡{n}≡)
-    ) vertex_wp.
-  Proof.
-    intros t t_ <- γ γ_ <-.
-    induction (lt_wf n) as [n _ IH] => P1 P2 HP R1 R2 HR task task_ <- gen gen_ <-.
-    rewrite !vertex_wp_unfold /vertex_wp_body.
-    do 16 f_equiv. f_contractive.
-    apply (dist_le _ m) in HP; last by apply SIdx.lt_le_incl.
-    apply (dist_le _ m) in HR; last by apply SIdx.lt_le_incl.
-    do 3 f_equiv; last solve_proper.
-    apply IH; done.
-  Qed.
-
-  #[local] Definition inv_state_init preds gen Π : iProp Σ :=
-    ∃ Δ,
-    dependencies_auth gen Own (Δ ⊎ Π) ∗
-    ⌜preds = S (size Π)⌝ ∗
-    [∗ mset] δ ∈ Δ, vertex_finished δ.
-  #[local] Instance : CustomIpatFormat "inv_state_init" :=
-    "(
-      %Δ &
-      {>;}Hdependencies{which;}_auth &
-      {>;}-> &
-      {>;}HΔ
-    )".
-  #[local] Definition inv_state_released t γ P R preds gen Π : iProp Σ :=
-    ∃ task Δ,
-    model' t γ task Released gen ∗
-    dependencies_auth gen Discard (Δ ⊎ Π) ∗
-    ⌜preds = size Π⌝ ∗
-    ([∗ mset] δ ∈ Δ, vertex_finished δ) ∗
-    vertex_wp t γ P R task gen.
-  #[local] Instance : CustomIpatFormat "inv_state_released" :=
-    "(
-      %task &
-      %Δ &
-      (:model' {//} {/which/}) &
-      {>;}Hdependencies{which;}_auth &
-      {>;}-> &
-      {>;}HΔ &
-      Htask
-    )".
-  #[local] Definition inv_state_running Π : iProp Σ :=
-    ⌜Π = ∅⌝.
-  #[local] Instance : CustomIpatFormat "inv_state_running" :=
-    "{>;}->".
-  #[local] Definition inv_state_finished γ R preds Π : iProp Σ :=
-    vertex_finished γ ∗
-    ⌜preds = S (size Π)⌝ ∗
-    □ R.
-  #[local] Instance : CustomIpatFormat "inv_state_finished" :=
-    "(
-      {>;}#Hstate{which;}₁ &
-      {>;}-> &
-      #HR{which;}
-    )".
-  #[local] Definition inv_state t γ P R state preds gen Π : iProp Σ :=
-    match state with
-    | Init =>
-        inv_state_init preds gen Π
-    | Released =>
-        inv_state_released t γ P R preds gen Π
-    | Running =>
-        inv_state_running Π
-    | Finished =>
-        inv_state_finished γ R preds Π
-    end.
-
-  #[local] Definition inv_successor (inv : location → vertex_name → iProp Σ → iProp Σ → iProp Σ) γ succ : iProp Σ :=
-    ∃ γ_succ P_succ R_succ,
-    inv succ γ_succ P_succ R_succ ∗
-    predecessors_elem γ_succ γ.
-  #[local] Instance : CustomIpatFormat "inv_successor" :=
-    "(
-      %γ_succ &
-      %P_succ &
-      %R_succ &
-      #Hinv_succ &
-      Hpredecessors_elem
-    )".
-  #[local] Definition inv_successors inv γ finished :=
-    if finished then (
-      mpmc_stack_2_model γ.(vertex_name_successors) None
-    ) else (
-      ∃ succs,
-      mpmc_stack_2_model γ.(vertex_name_successors) (Some $ #@{location} <$> succs) ∗
-      [∗ list] succ ∈ succs, inv_successor inv γ succ
-    )%I.
-  #[local] Instance : CustomIpatFormat "inv_successors_finished" :=
-    ">Hsuccessors{which;}_model".
-  #[local] Instance : CustomIpatFormat "inv_successors" :=
-    "(
-      %succs &
-      >Hsuccessors{which;}_model &
-      Hsuccs
-    )".
-
-  #[local] Definition inv_inner inv t γ P R : iProp Σ :=
-    ∃ preds state gen Π,
-    t.[preds] ↦ #preds ∗
-    state₂ γ state ∗
-    generation₂ γ gen ∗
-    predecessors_auth γ Π ∗
-    output_auth γ P (bool_decide (state = Finished)) ∗
-    inv_state t γ P R state preds gen Π ∗
-    inv_successors inv γ (bool_decide (state = Finished)).
-  #[local] Instance : CustomIpatFormat "inv_inner" :=
-    "(
-      %preds{} &
-      %state{} &
-      %gen{} &
-      %Π &
-      Ht{which;}_preds &
-      >Hstate{which;}₂ &
-      >Hgeneration{which;}₂ &
-      Hpredecessors{which;}_auth &
-      Houtput{which;}_auth &
-      Hinv_state{which;} &
-      Hinv_successors{which;}
-    )".
-  #[local] Definition inv_pre
-  : (location -d> vertex_name -d> iProp Σ -d> iProp Σ -d> iProp Σ) →
-    location -d> vertex_name -d> iProp Σ -d> iProp Σ -d> iProp Σ
-  :=
-    λ inv t γ P R, (
-      t.[succs] ↦□ γ.(vertex_name_successors) ∗
-      mpmc_stack_2_inv γ.(vertex_name_successors) (nroot.@"successors") ∗
-      invariants.inv (nroot.@"inv") (inv_inner inv t γ P R)
-    )%I.
-  #[local] Instance : CustomIpatFormat "inv_pre" :=
-    "(
-      #Ht{}_succs &
-      #Hsuccessors{}_inv &
-      #Hinv{_{}}
-    )".
-  #[local] Instance inv_pre_contractive_2 :
-    Contractive inv_pre.
-  Proof.
-    rewrite /inv_pre /inv_inner /inv_successors /inv_successor.
-    intros n Ψ1 Ψ2 HΨ t γ P R.
-    repeat (apply HΨ || f_contractive || f_equiv).
-  Qed.
-  Definition vertex_inv : location → vertex_name → iProp Σ → iProp Σ → iProp Σ :=
-    fixpoint inv_pre.
-
-  #[local] Lemma vertex_inv_unfold t γ P R :
-    vertex_inv t γ P R ⊣⊢
-    inv_pre vertex_inv t γ P R.
-  Proof.
-    apply (fixpoint_unfold inv_pre).
-  Qed.
-  #[local] Instance vertex_inv_contractive t γ n :
-    Proper (
-      dist_later n ==>
-      dist_later n ==>
-      (≡{n}≡)
-    ) (vertex_inv t γ).
-  Proof.
-    induction (lt_wf n) as [n _ IH] => P1 P2 HP R1 R2 HR.
-    rewrite !vertex_inv_unfold /inv_pre /inv_inner /inv_state /inv_state_released /inv_state_finished /inv_successors /inv_successor.
-    solve_contractive.
-  Qed.
-  #[global] Instance vertex_inv_ne t γ n :
-    Proper (
-      (≡{n}≡) ==>
-      (≡{n}≡) ==>
-      (≡{n}≡)
-    ) (vertex_inv t γ).
-  Proof.
-    intros P1 P2 HP R1 R2 HR.
-    apply vertex_inv_contractive.
-    all: apply dist_dist_later; done.
-  Qed.
-  #[global] Instance vertex_inv_proper t γ :
-    Proper (
-      (≡) ==>
-      (≡) ==>
-      (≡)
-    ) (vertex_inv t γ).
-  Proof.
-    intros P1 P2 HP R1 R2 HR.
-    rewrite !equiv_dist in HP HR |- * => n.
-    apply vertex_inv_ne; done.
-  Qed.
-
-  Definition vertex_output γ Q :=
-    output_frag γ Q.
-  #[local] Instance : CustomIpatFormat "output" :=
-    "Houtput{which;}_frag{_{}}".
-
-  #[global] Instance vertex_output_contractive γ :
-    Contractive (vertex_output γ).
-  Proof.
-    solve_contractive.
-  Qed.
-  #[global] Instance vertex_output_proper γ :
-    Proper ((≡) ==> (≡)) (vertex_output γ).
-  Proof.
-    solve_proper.
-  Qed.
-
-  Definition vertex_predecessor γ gen :=
-    dependencies_elem gen γ.
-  #[local] Instance : CustomIpatFormat "predecessor" :=
-    "#Hdependencies{which;}_elem{_{}}".
-
-  #[global] Instance vertex_model_timeless t γ task gen :
-    Timeless (vertex_model t γ task gen).
-  Proof.
-    apply _.
-  Qed.
-  #[global] Instance vertex_running_timeless gen :
-    Timeless (vertex_running gen).
-  Proof.
-    apply _.
-  Qed.
-  #[global] Instance vertex_finished_timeless γ :
-    Timeless (vertex_finished γ).
-  Proof.
-    apply _.
-  Qed.
-  #[global] Instance vertex_predecessor_timeless γ gen :
-    Timeless (vertex_predecessor γ gen).
-  Proof.
-    apply _.
-  Qed.
-
-  #[global] Instance vertex_inv_persistent t γ P R :
-    Persistent (vertex_inv t γ P R).
-  Proof.
-    rewrite vertex_inv_unfold.
-    apply _.
-  Qed.
-  #[global] Instance vertex_running_persistent gen :
-    Persistent (vertex_running gen).
-  Proof.
-    apply _.
-  Qed.
-  #[global] Instance vertex_finished_persistent γ :
-    Persistent (vertex_finished γ).
-  Proof.
-    apply _.
-  Qed.
-  #[global] Instance vertex_predecessor_persistent γ gen :
-    Persistent (vertex_predecessor γ gen).
-  Proof.
-    apply _.
-  Qed.
-
-  #[local] Lemma state_alloc :
-    ⊢ |==>
-      ∃ γ_state,
-      state₁' γ_state Own Init ∗
-      state₂' γ_state Init.
-  Proof.
-    apply twins_alloc'.
-  Qed.
-  #[local] Lemma state_agree γ own1 state1 state2 :
-    state₁ γ own1 state1 -∗
-    state₂ γ state2 -∗
-    ⌜state1 = state2⌝.
-  Proof.
-    apply: twins_agree_L.
-  Qed.
-  #[local] Lemma state₁_exclusive γ state1 own2 state2 :
-    state₁ γ Own state1 -∗
-    state₁ γ own2 state2 -∗
-    False.
-  Proof.
-    apply twins_twin1_exclusive.
-  Qed.
-  #[local] Lemma state_update {γ state1 state2} state :
-    state₁ γ Own state1 -∗
-    state₂ γ state2 ==∗
+    #[local] Definition model' t γ task state gen : iProp Σ :=
+      t.[task] ↦ task ∗
       state₁ γ Own state ∗
-      state₂ γ state.
-  Proof.
-    apply twins_update.
-  Qed.
-  #[local] Lemma state₁_discard γ state :
-    state₁ γ Own state ⊢ |==>
-    state₁ γ Discard state.
-  Proof.
-    apply twins_twin1_persist.
-  Qed.
+      generation₁ γ gen.
+    #[local] Instance : CustomIpatFormat "model'" :=
+      "(
+        Ht{which;}_task{_{}} &
+        Hstate{which;}₁{_{}} &
+        Hgeneration{which;}₁{_{}}
+      )".
+    Definition vertex_model t γ task gen : iProp Σ :=
+      model' t γ task Init gen.
+    #[local] Instance : CustomIpatFormat "model" :=
+      "(:model' {//} {/which/})".
 
-  #[local] Lemma generation_alloc gen :
-    ⊢ |==>
-      ∃ γ_generation,
-      generation₁' γ_generation gen ∗
-      generation₂' γ_generation gen.
-  Proof.
-    apply twins_alloc'.
-  Qed.
-  #[local] Lemma generation_agree γ generation1 generation2 :
-    generation₁ γ generation1 -∗
-    generation₂ γ generation2 -∗
-    ⌜generation1 = generation2⌝.
-  Proof.
-    apply: twins_agree_L.
-  Qed.
-  #[local] Lemma generation₁_exclusive γ generation1 generation2 :
-    generation₁ γ generation1 -∗
-    generation₁ γ generation2 -∗
-    False.
-  Proof.
-    apply twins_twin1_exclusive.
-  Qed.
-  #[local] Lemma generation_update {γ generation1 generation2} generation :
-    generation₁ γ generation1 -∗
-    generation₂ γ generation2 ==∗
-      generation₁ γ generation ∗
-      generation₂ γ generation.
-  Proof.
-    apply twins_update.
-  Qed.
+    Definition vertex_running gen : iProp Σ :=
+      ∃ Δ,
+      dependencies_auth gen Discard Δ ∗
+      [∗ mset] δ ∈ Δ, state₁ δ Discard Finished.
+    #[local] Instance : CustomIpatFormat "running" :=
+      "(
+        %Δ{} &
+        #Hdependencies{which;}_auth{_{}} &
+        #HΔ{}
+      )".
 
-  #[local] Lemma dependencies_alloc :
-    ⊢ |==>
-      ∃ gen,
-      dependencies_auth gen Own ∅.
-  Proof.
-    apply mono_gmultiset_alloc.
-  Qed.
-  #[local] Lemma dependencies_add {gen Δ} δ :
-    dependencies_auth gen Own Δ ⊢ |==>
-      dependencies_auth gen Own ({[+δ+]} ⊎ Δ) ∗
-      dependencies_elem gen δ.
-  Proof.
-    apply mono_gmultiset_insert'.
-  Qed.
-  #[local] Lemma dependencies_elem_of gen own Δ δ :
-    dependencies_auth gen own Δ -∗
-    dependencies_elem gen δ -∗
-    ⌜δ ∈ Δ⌝.
-  Proof.
-    apply mono_gmultiset_elem_valid.
-  Qed.
-  #[local] Lemma dependencies_discard gen Δ :
-    dependencies_auth gen Own Δ ⊢ |==>
-    dependencies_auth gen Discard Δ.
-  Proof.
-    apply mono_gmultiset_auth_persist.
-  Qed.
+    Definition vertex_finished γ :=
+      state₁ γ Discard Finished.
+    #[local] Instance : CustomIpatFormat "finished" :=
+      "#Hstate{which;}₁{_{}}".
 
-  #[local] Lemma predecessors_alloc :
-    ⊢ |==>
-      ∃ γ_predecessors,
-      predecessors_auth' γ_predecessors ∅.
-  Proof.
-    apply auth_gmultiset_alloc.
-  Qed.
-  #[local] Lemma predecessors_elem_of γ Π π :
-    predecessors_auth γ Π -∗
-    predecessors_elem γ π -∗
-    ⌜π ∈ Π⌝.
-  Proof.
-    apply auth_gmultiset_elem_of.
-  Qed.
-  #[local] Lemma predecessors_add {γ Π} π :
-    predecessors_auth γ Π ⊢ |==>
-      predecessors_auth γ ({[+π+]} ⊎ Π) ∗
-      predecessors_elem γ π.
-  Proof.
-    apply auth_gmultiset_update_alloc_singleton.
-  Qed.
-  #[local] Lemma predecessors_remove γ Π π :
-    predecessors_auth γ Π -∗
-    predecessors_elem γ π ==∗
-    predecessors_auth γ (Π ∖ {[+π+]}).
-  Proof.
-    apply auth_gmultiset_update_dealloc.
-  Qed.
+    Definition vertex_wp_body t γ P R body task gen : iProp Σ :=
+      ∀ pool ctx gen',
+      pool_context pool ctx -∗
+      vertex_running gen -∗
+      vertex_model t γ task gen' -∗
+      WP task ctx {{ res,
+        ∃ b task,
+        ⌜res = #b⌝ ∗
+        ▷ (
+          pool_context pool ctx ∗
+          vertex_model t γ task gen' ∗
+          if b then
+            body task gen'
+          else
+            P ∗
+            □ R
+        )
+      }}.
+    #[local] Definition vertex_wp_pre
+    : location → vertex_name → iProp Σ → iProp Σ →
+      (val -d> vertex_generation -d> iProp Σ) →
+      val -d> vertex_generation -d> iProp Σ
+    :=
+      vertex_wp_body.
+    #[local] Instance vertex_wp_pre_contractive t γ P R :
+      Contractive (vertex_wp_pre t γ P R).
+    Proof.
+      rewrite /vertex_wp_pre /vertex_wp_body.
+      solve_contractive.
+    Qed.
+    #[local] Instance vertex_wp_pre_ne t γ P R :
+      NonExpansive (vertex_wp_pre t γ P R).
+    Proof.
+      apply _.
+    Qed.
+    Definition vertex_wp t γ P R : val → vertex_generation → iProp Σ :=
+      fixpoint (vertex_wp_pre t γ P R).
 
-  #[local] Lemma output_alloc P :
-    ⊢ |==>
-      ∃ γ_output,
-      output_auth' γ_output P false ∗
-      output_frag' γ_output P.
-  Proof.
-    apply subprops_alloc.
-  Qed.
-  #[local] Lemma output_divide {γ P finished Q} Qs E :
-    ▷ output_auth γ P finished -∗
-    output_frag γ Q -∗
-    (Q -∗ [∗ list] Q ∈ Qs, Q) ={E}=∗
-      ▷ output_auth γ P finished ∗
-      [∗ list] Q ∈ Qs, output_frag γ Q.
-  Proof.
-    apply subprops_divide.
-  Qed.
-  #[local] Lemma output_produce γ P :
-    ▷ output_auth γ P false -∗
-    P -∗
-    ▷ output_auth γ P true.
-  Proof.
-    iIntros "Hauth HP".
-    iApply (subprops_produce with "Hauth [$HP]").
-  Qed.
-  #[local] Lemma output_consume γ P Q E :
-    ▷ output_auth γ P true -∗
-    output_frag γ Q ={E}=∗
-      ▷ output_auth γ P true ∗
-      ▷^2 Q.
-  Proof.
-    apply subprops_consume.
-  Qed.
+    Lemma vertex_wp_unfold t γ P R task gen :
+      vertex_wp t γ P R task gen ⊣⊢
+      vertex_wp_body t γ P R (vertex_wp t γ P R) task gen.
+    Proof.
+      apply (fixpoint_unfold (vertex_wp_pre t γ P R)).
+    Qed.
+    #[global] Instance vertex_wp_ne n :
+      Proper (
+        (=) ==>
+        (=) ==>
+        (≡{n}≡) ==>
+        (≡{n}≡) ==>
+        (≡{n}≡) ==>
+        (≡{n}≡) ==>
+        (≡{n}≡)
+      ) vertex_wp.
+    Proof.
+      intros t t_ <- γ γ_ <-.
+      induction (lt_wf n) as [n _ IH] => P1 P2 HP R1 R2 HR task task_ <- gen gen_ <-.
+      rewrite !vertex_wp_unfold /vertex_wp_body.
+      do 16 f_equiv. f_contractive.
+      apply (dist_le _ m) in HP; last by apply SIdx.lt_le_incl.
+      apply (dist_le _ m) in HR; last by apply SIdx.lt_le_incl.
+      do 3 f_equiv; last solve_proper.
+      apply IH; done.
+    Qed.
 
-  Lemma vertex_model_exclusive t γ task1 gen1 task2 gen2 :
-    vertex_model t γ task1 gen1 -∗
-    vertex_model t γ task2 gen2 -∗
-    False.
-  Proof.
-    iIntros "(:model =1) (:model =2)".
-    iApply (generation₁_exclusive with "Hgeneration₁_1 Hgeneration₁_2").
-  Qed.
-  Lemma vertex_model_not_finished t γ task gen :
-    vertex_model t γ task gen -∗
-    vertex_finished γ -∗
-    False.
-  Proof.
-    iIntros "(:model =1) (:finished =2)".
-    iApply (state₁_exclusive with "Hstate₁_1 Hstate₁_2").
-  Qed.
+    #[local] Definition inv_state_init preds gen Π : iProp Σ :=
+      ∃ Δ,
+      dependencies_auth gen Own (Δ ⊎ Π) ∗
+      ⌜preds = S (size Π)⌝ ∗
+      [∗ mset] δ ∈ Δ, vertex_finished δ.
+    #[local] Instance : CustomIpatFormat "inv_state_init" :=
+      "(
+        %Δ &
+        {>;}Hdependencies{which;}_auth &
+        {>;}-> &
+        {>;}HΔ
+      )".
+    #[local] Definition inv_state_released t γ P R preds gen Π : iProp Σ :=
+      ∃ task Δ,
+      model' t γ task Released gen ∗
+      dependencies_auth gen Discard (Δ ⊎ Π) ∗
+      ⌜preds = size Π⌝ ∗
+      ([∗ mset] δ ∈ Δ, vertex_finished δ) ∗
+      vertex_wp t γ P R task gen.
+    #[local] Instance : CustomIpatFormat "inv_state_released" :=
+      "(
+        %task &
+        %Δ &
+        (:model' {//} {/which/}) &
+        {>;}Hdependencies{which;}_auth &
+        {>;}-> &
+        {>;}HΔ &
+        Htask
+      )".
+    #[local] Definition inv_state_running Π : iProp Σ :=
+      ⌜Π = ∅⌝.
+    #[local] Instance : CustomIpatFormat "inv_state_running" :=
+      "{>;}->".
+    #[local] Definition inv_state_finished γ R preds Π : iProp Σ :=
+      vertex_finished γ ∗
+      ⌜preds = S (size Π)⌝ ∗
+      □ R.
+    #[local] Instance : CustomIpatFormat "inv_state_finished" :=
+      "(
+        {>;}#Hstate{which;}₁ &
+        {>;}-> &
+        #HR{which;}
+      )".
+    #[local] Definition inv_state t γ P R state preds gen Π : iProp Σ :=
+      match state with
+      | Init =>
+          inv_state_init preds gen Π
+      | Released =>
+          inv_state_released t γ P R preds gen Π
+      | Running =>
+          inv_state_running Π
+      | Finished =>
+          inv_state_finished γ R preds Π
+      end.
 
-  Lemma vertex_output_divide {t γ P R Q} Qs :
-    vertex_inv t γ P R -∗
-    vertex_output γ Q -∗
-    (Q -∗ [∗ list] Q ∈ Qs, Q) ={⊤}=∗
-    [∗ list] Q ∈ Qs, vertex_output γ Q.
-  Proof.
-    rewrite vertex_inv_unfold.
-    iIntros "(:inv_pre) (:output) H".
-    iInv "Hinv" as "(:inv_inner)".
-    iMod (output_divide with "Houtput_auth Houtput_frag H") as "(Houtput_auth & H)".
-    iSplitR "H". { iFrameSteps. }
-    iApply (big_sepL_impl with "H").
-    iSteps.
-  Qed.
-  Lemma vertex_output_split {t γ P R Q} Q1 Q2 :
-    vertex_inv t γ P R -∗
-    vertex_output γ Q -∗
-    (Q -∗ Q1 ∗ Q2) ={⊤}=∗
-      vertex_output γ Q1 ∗
-      vertex_output γ Q2.
-  Proof.
-    iIntros "#Hinv Houtput H".
-    iMod (vertex_output_divide [Q1;Q2] with "Hinv Houtput [H]") as "($ & $ & _)"; iSteps.
-  Qed.
+    #[local] Definition inv_successor (inv : location → vertex_name → iProp Σ → iProp Σ → iProp Σ) γ succ : iProp Σ :=
+      ∃ γ_succ P_succ R_succ,
+      inv succ γ_succ P_succ R_succ ∗
+      predecessors_elem γ_succ γ.
+    #[local] Instance : CustomIpatFormat "inv_successor" :=
+      "(
+        %γ_succ &
+        %P_succ &
+        %R_succ &
+        #Hinv_succ &
+        Hpredecessors_elem
+      )".
+    #[local] Definition inv_successors inv γ finished :=
+      if finished then (
+        mpmc_stack_2_model γ.(vertex_name_successors) None
+      ) else (
+        ∃ succs,
+        mpmc_stack_2_model γ.(vertex_name_successors) (Some $ #@{location} <$> succs) ∗
+        [∗ list] succ ∈ succs, inv_successor inv γ succ
+      )%I.
+    #[local] Instance : CustomIpatFormat "inv_successors_finished" :=
+      ">Hsuccessors{which;}_model".
+    #[local] Instance : CustomIpatFormat "inv_successors" :=
+      "(
+        %succs &
+        >Hsuccessors{which;}_model &
+        Hsuccs
+      )".
 
-  Lemma vertex_predecessor_finished γ gen :
-    vertex_predecessor γ gen -∗
-    vertex_running gen -∗
-    vertex_finished γ.
-  Proof.
-    iIntros "(:predecessor) (:running)".
-    iDestruct (dependencies_elem_of with "Hdependencies_auth Hdependencies_elem") as %Hγ.
-    iDestruct (big_sepMS_elem_of with "HΔ") as "#Hstate₁"; first done.
-    iSteps.
-  Qed.
+    #[local] Definition inv_inner inv t γ P R : iProp Σ :=
+      ∃ preds state gen Π,
+      t.[preds] ↦ #preds ∗
+      state₂ γ state ∗
+      generation₂ γ gen ∗
+      predecessors_auth γ Π ∗
+      output_auth γ P (bool_decide (state = Finished)) ∗
+      inv_state t γ P R state preds gen Π ∗
+      inv_successors inv γ (bool_decide (state = Finished)).
+    #[local] Instance : CustomIpatFormat "inv_inner" :=
+      "(
+        %preds{} &
+        %state{} &
+        %gen{} &
+        %Π &
+        Ht{which;}_preds &
+        >Hstate{which;}₂ &
+        >Hgeneration{which;}₂ &
+        Hpredecessors{which;}_auth &
+        Houtput{which;}_auth &
+        Hinv_state{which;} &
+        Hinv_successors{which;}
+      )".
+    #[local] Definition inv_pre
+    : (location -d> vertex_name -d> iProp Σ -d> iProp Σ -d> iProp Σ) →
+      location -d> vertex_name -d> iProp Σ -d> iProp Σ -d> iProp Σ
+    :=
+      λ inv t γ P R, (
+        t.[succs] ↦□ γ.(vertex_name_successors) ∗
+        mpmc_stack_2_inv γ.(vertex_name_successors) (nroot.@"successors") ∗
+        invariants.inv (nroot.@"inv") (inv_inner inv t γ P R)
+      )%I.
+    #[local] Instance : CustomIpatFormat "inv_pre" :=
+      "(
+        #Ht{}_succs &
+        #Hsuccessors{}_inv &
+        #Hinv{_{}}
+      )".
+    #[local] Instance inv_pre_contractive_2 :
+      Contractive inv_pre.
+    Proof.
+      rewrite /inv_pre /inv_inner /inv_successors /inv_successor.
+      intros n Ψ1 Ψ2 HΨ t γ P R.
+      repeat (apply HΨ || f_contractive || f_equiv).
+    Qed.
+    Definition vertex_inv : location → vertex_name → iProp Σ → iProp Σ → iProp Σ :=
+      fixpoint inv_pre.
 
-  Lemma vertex_inv_finished t γ P R :
-    vertex_inv t γ P R -∗
-    vertex_finished γ ={⊤}=∗
-    ▷ □ R.
-  Proof.
-    setoid_rewrite vertex_inv_unfold.
-    iIntros "(:inv_pre) (:finished)".
-    iInv "Hinv" as "(:inv_inner)".
-    iDestruct (state_agree with "Hstate₁ Hstate₂") as %<-.
-    iDestruct "Hinv_state" as "{Hstate₁} (:inv_state_finished >)".
-    iSplitL. { iFrameSteps. }
-    iSteps.
-  Qed.
-  Lemma vertex_inv_finished' t γ P R :
-    £ 1 -∗
-    vertex_inv t γ P R -∗
-    vertex_finished γ ={⊤}=∗
-    □ R.
-  Proof.
-    iIntros "H£ Hinv Hfinished".
-    iMod (vertex_inv_finished with "Hinv Hfinished") as "HR".
-    iApply (lc_fupd_elim_later with "H£ HR").
-  Qed.
-  Lemma vertex_inv_finished_output t γ P R Q :
-    vertex_inv t γ P R -∗
-    vertex_finished γ -∗
-    vertex_output γ Q ={⊤}=∗
-    ▷^2 Q.
-  Proof.
-    setoid_rewrite vertex_inv_unfold.
-    iIntros "(:inv_pre) (:finished) (:output)".
-    iInv "Hinv" as "(:inv_inner)".
-    iDestruct (state_agree with "Hstate₁ Hstate₂") as %<-.
-    iMod (output_consume with "Houtput_auth Houtput_frag") as "(Houtput_auth & HP)".
-    iSplitR "HP". { iFrameSteps. }
-    iSteps.
-  Qed.
-  Lemma vertex_inv_finished_output' t γ P R Q :
-    £ 2 -∗
-    vertex_inv t γ P R -∗
-    vertex_finished γ -∗
-    vertex_output γ Q ={⊤}=∗
-    Q.
-  Proof.
-    iIntros "(H£1 & H£2) Hinv Hfinished Houtput".
-    iMod (vertex_inv_finished_output with "Hinv Hfinished Houtput") as "HP".
-    iMod (lc_fupd_elim_later with "H£1 HP") as "HP".
-    iApply (lc_fupd_elim_later with "H£2 HP").
-  Qed.
+    #[local] Lemma vertex_inv_unfold t γ P R :
+      vertex_inv t γ P R ⊣⊢
+      inv_pre vertex_inv t γ P R.
+    Proof.
+      apply (fixpoint_unfold inv_pre).
+    Qed.
+    #[local] Instance vertex_inv_contractive t γ n :
+      Proper (
+        dist_later n ==>
+        dist_later n ==>
+        (≡{n}≡)
+      ) (vertex_inv t γ).
+    Proof.
+      induction (lt_wf n) as [n _ IH] => P1 P2 HP R1 R2 HR.
+      rewrite !vertex_inv_unfold /inv_pre /inv_inner /inv_state /inv_state_released /inv_state_finished /inv_successors /inv_successor.
+      solve_contractive.
+    Qed.
+    #[global] Instance vertex_inv_ne t γ n :
+      Proper (
+        (≡{n}≡) ==>
+        (≡{n}≡) ==>
+        (≡{n}≡)
+      ) (vertex_inv t γ).
+    Proof.
+      intros P1 P2 HP R1 R2 HR.
+      apply vertex_inv_contractive.
+      all: apply dist_dist_later; done.
+    Qed.
+    #[global] Instance vertex_inv_proper t γ :
+      Proper (
+        (≡) ==>
+        (≡) ==>
+        (≡)
+      ) (vertex_inv t γ).
+    Proof.
+      intros P1 P2 HP R1 R2 HR.
+      rewrite !equiv_dist in HP HR |- * => n.
+      apply vertex_inv_ne; done.
+    Qed.
 
-  Lemma vertex_create_spec P R (task : option val) :
-    {{{
-      True
-    }}}
-      vertex_create task
-    {{{ t γ gen,
-      RET #t;
-      vertex_inv t γ P R ∗
-      vertex_model t γ (default (fun: <> => #false)%V task) gen ∗
-      vertex_output γ P
-    }}}.
-  Proof.
-    iIntros "%Φ _ HΦ".
+    Definition vertex_output γ Q :=
+      output_frag γ Q.
+    #[local] Instance : CustomIpatFormat "output" :=
+      "Houtput{which;}_frag{_{}}".
 
-    wp_rec.
+    #[global] Instance vertex_output_contractive γ :
+      Contractive (vertex_output γ).
+    Proof.
+      solve_contractive.
+    Qed.
+    #[global] Instance vertex_output_proper γ :
+      Proper ((≡) ==> (≡)) (vertex_output γ).
+    Proof.
+      solve_proper.
+    Qed.
 
-    wp_bind (Match _ _ _ _).
-    wp_apply (wp_wand (λ res,
-      ⌜res = default (fun: <> => #false)%V task⌝
-    )%I) as (res) "->".
-    { destruct task; iSteps. }
+    Definition vertex_predecessor γ gen :=
+      dependencies_elem gen γ.
+    #[local] Instance : CustomIpatFormat "predecessor" :=
+      "#Hdependencies{which;}_elem{_{}}".
 
-    wp_smart_apply (mpmc_stack_2_create_spec with "[//]") as (succs) "(#Hsuccessors_inv & Hsuccessors_model)".
-    wp_block t as "(Ht_task & Ht_preds & Ht_succs & _)".
-    iMod (pointsto_persist with "Ht_succs") as "#Ht_succs".
+    #[global] Instance vertex_model_timeless t γ task gen :
+      Timeless (vertex_model t γ task gen).
+    Proof.
+      apply _.
+    Qed.
+    #[global] Instance vertex_running_timeless gen :
+      Timeless (vertex_running gen).
+    Proof.
+      apply _.
+    Qed.
+    #[global] Instance vertex_finished_timeless γ :
+      Timeless (vertex_finished γ).
+    Proof.
+      apply _.
+    Qed.
+    #[global] Instance vertex_predecessor_timeless γ gen :
+      Timeless (vertex_predecessor γ gen).
+    Proof.
+      apply _.
+    Qed.
 
-    iMod state_alloc as "(%γ_state & Hstate₁ & Hstate₂)".
-    iMod dependencies_alloc as "(%gen & Hdependencies_auth)".
-    iMod (generation_alloc gen) as "(%γ_generation & Hgeneration₁ & Hgeneration₂)".
-    iMod predecessors_alloc as "(%γ_predecessors & Hpredecessors_auth)".
-    iMod (output_alloc P) as "(%γ_output & Houtput_auth & Houtput_frag)".
+    #[global] Instance vertex_inv_persistent t γ P R :
+      Persistent (vertex_inv t γ P R).
+    Proof.
+      rewrite vertex_inv_unfold.
+      apply _.
+    Qed.
+    #[global] Instance vertex_running_persistent gen :
+      Persistent (vertex_running gen).
+    Proof.
+      apply _.
+    Qed.
+    #[global] Instance vertex_finished_persistent γ :
+      Persistent (vertex_finished γ).
+    Proof.
+      apply _.
+    Qed.
+    #[global] Instance vertex_predecessor_persistent γ gen :
+      Persistent (vertex_predecessor γ gen).
+    Proof.
+      apply _.
+    Qed.
 
-    pose γ := {|
-      vertex_name_successors := succs ;
-      vertex_name_state := γ_state ;
-      vertex_name_generation := γ_generation ;
-      vertex_name_predecessors := γ_predecessors ;
-      vertex_name_output := γ_output ;
-    |}.
+    #[local] Lemma state_alloc :
+      ⊢ |==>
+        ∃ γ_state,
+        state₁' γ_state Own Init ∗
+        state₂' γ_state Init.
+    Proof.
+      apply twins_alloc'.
+    Qed.
+    #[local] Lemma state_agree γ own1 state1 state2 :
+      state₁ γ own1 state1 -∗
+      state₂ γ state2 -∗
+      ⌜state1 = state2⌝.
+    Proof.
+      apply: twins_agree_L.
+    Qed.
+    #[local] Lemma state₁_exclusive γ state1 own2 state2 :
+      state₁ γ Own state1 -∗
+      state₁ γ own2 state2 -∗
+      False.
+    Proof.
+      apply twins_twin1_exclusive.
+    Qed.
+    #[local] Lemma state_update {γ state1 state2} state :
+      state₁ γ Own state1 -∗
+      state₂ γ state2 ==∗
+        state₁ γ Own state ∗
+        state₂ γ state.
+    Proof.
+      apply twins_update.
+    Qed.
+    #[local] Lemma state₁_discard γ state :
+      state₁ γ Own state ⊢ |==>
+      state₁ γ Discard state.
+    Proof.
+      apply twins_twin1_persist.
+    Qed.
 
-    iApply ("HΦ" $! t γ).
-    iSplitR "Ht_task Hstate₁ Hgeneration₁ Houtput_frag"; last iSteps.
-    rewrite vertex_inv_unfold. iStep 2.
-    iApply inv_alloc.
-    iExists 1, Init, gen, ∅. iFrame. iSplitR "Hsuccessors_model".
-    - rewrite /inv_state /inv_state_init.
-      iExists ∅. rewrite big_sepMS_empty left_id. iSteps.
-    - iExists []. iSteps.
-  Qed.
+    #[local] Lemma generation_alloc gen :
+      ⊢ |==>
+        ∃ γ_generation,
+        generation₁' γ_generation gen ∗
+        generation₂' γ_generation gen.
+    Proof.
+      apply twins_alloc'.
+    Qed.
+    #[local] Lemma generation_agree γ generation1 generation2 :
+      generation₁ γ generation1 -∗
+      generation₂ γ generation2 -∗
+      ⌜generation1 = generation2⌝.
+    Proof.
+      apply: twins_agree_L.
+    Qed.
+    #[local] Lemma generation₁_exclusive γ generation1 generation2 :
+      generation₁ γ generation1 -∗
+      generation₁ γ generation2 -∗
+      False.
+    Proof.
+      apply twins_twin1_exclusive.
+    Qed.
+    #[local] Lemma generation_update {γ generation1 generation2} generation :
+      generation₁ γ generation1 -∗
+      generation₂ γ generation2 ==∗
+        generation₁ γ generation ∗
+        generation₂ γ generation.
+    Proof.
+      apply twins_update.
+    Qed.
 
-  Lemma vertex_task_spec t γ task gen :
-    {{{
-      vertex_model t γ task gen
-    }}}
-      vertex_task #t
-    {{{
-      RET task;
-      vertex_model t γ task gen
-    }}}.
-  Proof.
-    iSteps.
-  Qed.
+    #[local] Lemma dependencies_alloc :
+      ⊢ |==>
+        ∃ gen,
+        dependencies_auth gen Own ∅.
+    Proof.
+      apply mono_gmultiset_alloc.
+    Qed.
+    #[local] Lemma dependencies_add {gen Δ} δ :
+      dependencies_auth gen Own Δ ⊢ |==>
+        dependencies_auth gen Own ({[+δ+]} ⊎ Δ) ∗
+        dependencies_elem gen δ.
+    Proof.
+      apply mono_gmultiset_insert'.
+    Qed.
+    #[local] Lemma dependencies_elem_of gen own Δ δ :
+      dependencies_auth gen own Δ -∗
+      dependencies_elem gen δ -∗
+      ⌜δ ∈ Δ⌝.
+    Proof.
+      apply mono_gmultiset_elem_valid.
+    Qed.
+    #[local] Lemma dependencies_discard gen Δ :
+      dependencies_auth gen Own Δ ⊢ |==>
+      dependencies_auth gen Discard Δ.
+    Proof.
+      apply mono_gmultiset_auth_persist.
+    Qed.
 
-  Lemma vertex_set_task_spec t γ task1 gen task2 :
-    {{{
-      vertex_model t γ task1 gen
-    }}}
-      vertex_set_task #t task2
-    {{{
-      RET ();
-      vertex_model t γ task2 gen
-    }}}.
-  Proof.
-    iSteps.
-  Qed.
+    #[local] Lemma predecessors_alloc :
+      ⊢ |==>
+        ∃ γ_predecessors,
+        predecessors_auth' γ_predecessors ∅.
+    Proof.
+      apply auth_gmultiset_alloc.
+    Qed.
+    #[local] Lemma predecessors_elem_of γ Π π :
+      predecessors_auth γ Π -∗
+      predecessors_elem γ π -∗
+      ⌜π ∈ Π⌝.
+    Proof.
+      apply auth_gmultiset_elem_of.
+    Qed.
+    #[local] Lemma predecessors_add {γ Π} π :
+      predecessors_auth γ Π ⊢ |==>
+        predecessors_auth γ ({[+π+]} ⊎ Π) ∗
+        predecessors_elem γ π.
+    Proof.
+      apply auth_gmultiset_update_alloc_singleton.
+    Qed.
+    #[local] Lemma predecessors_remove γ Π π :
+      predecessors_auth γ Π -∗
+      predecessors_elem γ π ==∗
+      predecessors_auth γ (Π ∖ {[+π+]}).
+    Proof.
+      apply auth_gmultiset_update_dealloc.
+    Qed.
 
-  Lemma vertex_set_task'_spec t γ task1 gen task2 :
-    {{{
-      vertex_model t γ task1 gen
-    }}}
-      vertex_set_task' #t task2
-    {{{
-      RET ();
-      vertex_model t γ (fun: "ctx" => task2 "ctx" ;; #false) gen
-    }}}.
-  Proof.
-    iIntros "%Φ Hmodel HΦ".
+    #[local] Lemma output_alloc P :
+      ⊢ |==>
+        ∃ γ_output,
+        output_auth' γ_output P false ∗
+        output_frag' γ_output P.
+    Proof.
+      apply subprops_alloc.
+    Qed.
+    #[local] Lemma output_divide {γ P finished Q} Qs E :
+      ▷ output_auth γ P finished -∗
+      output_frag γ Q -∗
+      (Q -∗ [∗ list] Q ∈ Qs, Q) ={E}=∗
+        ▷ output_auth γ P finished ∗
+        [∗ list] Q ∈ Qs, output_frag γ Q.
+    Proof.
+      apply subprops_divide.
+    Qed.
+    #[local] Lemma output_produce γ P :
+      ▷ output_auth γ P false -∗
+      P -∗
+      ▷ output_auth γ P true.
+    Proof.
+      iIntros "Hauth HP".
+      iApply (subprops_produce with "Hauth [$HP]").
+    Qed.
+    #[local] Lemma output_consume γ P Q E :
+      ▷ output_auth γ P true -∗
+      output_frag γ Q ={E}=∗
+        ▷ output_auth γ P true ∗
+        ▷^2 Q.
+    Proof.
+      apply subprops_consume.
+    Qed.
 
-    wp_rec.
-    wp_smart_apply (vertex_set_task_spec with "Hmodel HΦ").
-  Qed.
+    Lemma vertex_model_exclusive t γ task1 gen1 task2 gen2 :
+      vertex_model t γ task1 gen1 -∗
+      vertex_model t γ task2 gen2 -∗
+      False.
+    Proof.
+      iIntros "(:model =1) (:model =2)".
+      iApply (generation₁_exclusive with "Hgeneration₁_1 Hgeneration₁_2").
+    Qed.
+    Lemma vertex_model_finished t γ task gen :
+      vertex_model t γ task gen -∗
+      vertex_finished γ -∗
+      False.
+    Proof.
+      iIntros "(:model =1) (:finished =2)".
+      iApply (state₁_exclusive with "Hstate₁_1 Hstate₁_2").
+    Qed.
 
-  Lemma vertex_precede_spec t1 γ1 P1 R1 t2 γ2 P2 R2 task gen :
-    {{{
-      vertex_inv t1 γ1 P1 R1 ∗
-      vertex_inv t2 γ2 P2 R2 ∗
-      vertex_model t2 γ2 task gen
-    }}}
-      vertex_precede #t1 #t2
-    {{{
-      RET ();
-      vertex_model t2 γ2 task gen ∗
-      vertex_predecessor γ1 gen
-    }}}.
-  Proof.
-    setoid_rewrite vertex_inv_unfold.
-    iIntros "%Φ ((:inv_pre =1) & (:inv_pre =2) & (:model which=2)) HΦ".
-
-    wp_rec.
-    iApply (wp_frame_wand with "[Ht2_task HΦ]"); first iAccu.
-    wp_load.
-
-    awp_smart_apply (mpmc_stack_2_is_closed_spec with "Hsuccessors1_inv") without "Hstate2₁ Hgeneration2₁".
-    iInv "Hinv_1" as "(:inv_inner which=1 =1)".
-    case_decide as Hstate1; first subst.
-
-    - iDestruct "Hinv_state1" as "(:inv_state_finished which=1 =1 >) /=".
-      iDestruct "Hinv_successors1" as "(:inv_successors_finished which=1 =1)".
-      iAaccIntro with "Hsuccessors1_model"; iIntros "Hsuccs1_model !>".
-      { iFrameSteps. }
-      iSplitL. { iFrameSteps. }
-      iIntros "{%} _ (Hstate2₁ & Hgeneration2₁)".
-
-      iApply fupd_wp.
-      iInv "Hinv_2" as "(:inv_inner which=2 =1)".
-      iDestruct (state_agree with "Hstate2₁ Hstate2₂") as %<-.
-      iDestruct (generation_agree with "Hgeneration2₁ Hgeneration2₂") as %<-.
-      iDestruct "Hinv_state2" as "(:inv_state_init which=2 =1 >)".
-      iMod (dependencies_add γ1 with "Hdependencies2_auth") as "(Hdependencies2_auth & #Hdependencies2_elem)".
-      iDestruct (big_sepMS_insert_2 γ1 with "HΔ Hstate1₁") as "HΔ".
-      iSplitR "Hstate2₁ Hgeneration2₁".
-      { assert ({[+γ1+]} ⊎ (Δ ⊎ Π) = ({[+γ1+]} ⊎ Δ) ⊎ Π) as ->.
-        { rewrite assoc //. }
-        iFrame. rewrite /inv_state. iFrameSteps.
-      }
+    Lemma vertex_output_divide {t γ P R Q} Qs :
+      vertex_inv t γ P R -∗
+      vertex_output γ Q -∗
+      (Q -∗ [∗ list] Q ∈ Qs, Q) ={⊤}=∗
+      [∗ list] Q ∈ Qs, vertex_output γ Q.
+    Proof.
+      rewrite vertex_inv_unfold.
+      iIntros "(:inv_pre) (:output) H".
+      iInv "Hinv" as "(:inv_inner)".
+      iMod (output_divide with "Houtput_auth Houtput_frag H") as "(Houtput_auth & H)".
+      iSplitR "H". { iFrameSteps. }
+      iApply (big_sepL_impl with "H").
       iSteps.
+    Qed.
+    Lemma vertex_output_split {t γ P R Q} Q1 Q2 :
+      vertex_inv t γ P R -∗
+      vertex_output γ Q -∗
+      (Q -∗ Q1 ∗ Q2) ={⊤}=∗
+        vertex_output γ Q1 ∗
+        vertex_output γ Q2.
+    Proof.
+      iIntros "#Hinv Houtput H".
+      iMod (vertex_output_divide [Q1;Q2] with "Hinv Houtput [H]") as "($ & $ & _)"; iSteps.
+    Qed.
 
-    - iDestruct "Hinv_successors1" as "(:inv_successors which=1 =1)".
-      iAaccIntro with "Hsuccessors1_model"; iIntros "Hsuccs_model !>".
-      { iFrameSteps. rewrite bool_decide_eq_false_2 //. iSteps. }
-      iSplitL.
-      { iFrameSteps. rewrite bool_decide_eq_false_2 //. iSteps. }
-      iIntros "{%} _ (Hstate2₁ & Hgeneration2₁)".
+    Lemma vertex_predecessor_finished γ gen :
+      vertex_predecessor γ gen -∗
+      vertex_running gen -∗
+      vertex_finished γ.
+    Proof.
+      iIntros "(:predecessor) (:running)".
+      iDestruct (dependencies_elem_of with "Hdependencies_auth Hdependencies_elem") as %Hγ.
+      iDestruct (big_sepMS_elem_of with "HΔ") as "#Hstate₁"; first done.
+      iSteps.
+    Qed.
 
-      wp_pures.
+    Lemma vertex_inv_finished t γ P R :
+      vertex_inv t γ P R -∗
+      vertex_finished γ ={⊤}=∗
+      ▷ □ R.
+    Proof.
+      setoid_rewrite vertex_inv_unfold.
+      iIntros "(:inv_pre) (:finished)".
+      iInv "Hinv" as "(:inv_inner)".
+      iDestruct (state_agree with "Hstate₁ Hstate₂") as %<-.
+      iDestruct "Hinv_state" as "{Hstate₁} (:inv_state_finished >)".
+      iSplitL. { iFrameSteps. }
+      iSteps.
+    Qed.
+    Lemma vertex_inv_finished' t γ P R :
+      £ 1 -∗
+      vertex_inv t γ P R -∗
+      vertex_finished γ ={⊤}=∗
+      □ R.
+    Proof.
+      iIntros "H£ Hinv Hfinished".
+      iMod (vertex_inv_finished with "Hinv Hfinished") as "HR".
+      iApply (lc_fupd_elim_later with "H£ HR").
+    Qed.
+    Lemma vertex_inv_finished_output t γ P R Q :
+      vertex_inv t γ P R -∗
+      vertex_finished γ -∗
+      vertex_output γ Q ={⊤}=∗
+      ▷^2 Q.
+    Proof.
+      setoid_rewrite vertex_inv_unfold.
+      iIntros "(:inv_pre) (:finished) (:output)".
+      iInv "Hinv" as "(:inv_inner)".
+      iDestruct (state_agree with "Hstate₁ Hstate₂") as %<-.
+      iMod (output_consume with "Houtput_auth Houtput_frag") as "(Houtput_auth & HP)".
+      iSplitR "HP". { iFrameSteps. }
+      iSteps.
+    Qed.
+    Lemma vertex_inv_finished_output' t γ P R Q :
+      £ 2 -∗
+      vertex_inv t γ P R -∗
+      vertex_finished γ -∗
+      vertex_output γ Q ={⊤}=∗
+      Q.
+    Proof.
+      iIntros "(H£1 & H£2) Hinv Hfinished Houtput".
+      iMod (vertex_inv_finished_output with "Hinv Hfinished Houtput") as "HP".
+      iMod (lc_fupd_elim_later with "H£1 HP") as "HP".
+      iApply (lc_fupd_elim_later with "H£2 HP").
+    Qed.
 
-      wp_bind (FAA _ _).
-      iInv "Hinv_2" as "(:inv_inner which=2 =1)".
-      wp_faa.
-      iDestruct (state_agree with "Hstate2₁ Hstate2₂") as %<-.
-      iDestruct (generation_agree with "Hgeneration2₁ Hgeneration2₂") as %<-.
-      iDestruct "Hinv_state2" as "(:inv_state_init which=2 =1)".
-      iMod (dependencies_add γ1 with "Hdependencies2_auth") as "(Hdependencies2_auth & #Hdependencies2_elem)".
-      iMod (predecessors_add γ1 with "Hpredecessors2_auth") as "(Hpredecessors2_auth & Hpredecessors2_elem )".
-      iSplitR "Hstate2₁ Hgeneration2₁ Hpredecessors2_elem".
-      { assert ({[+γ1+]} ⊎ (Δ ⊎ Π) = Δ ⊎ ({[+γ1+]} ⊎ Π)) as ->.
-        { rewrite assoc (comm _ _ Δ) -assoc //. }
-        iFrameSteps. iPureIntro.
-        rewrite gmultiset_size_disj_union gmultiset_size_singleton. lia.
-      }
-      iIntros "!> {%}".
+    Lemma vertex_create_spec P R (task : option val) :
+      {{{
+        True
+      }}}
+        vertex_create task
+      {{{ t γ gen,
+        RET #t;
+        meta_token t ⊤ ∗
+        vertex_inv t γ P R ∗
+        vertex_model t γ (default (fun: <> => #false)%V task) gen ∗
+        vertex_output γ P
+      }}}.
+    Proof.
+      iIntros "%Φ _ HΦ".
 
-      wp_pures. clear.
+      wp_rec.
 
-      awp_apply (mpmc_stack_2_push_spec with "Hsuccessors1_inv") without "Hstate2₁ Hgeneration2₁".
-      iInv "Hinv_1" as "(:inv_inner which=1 =2)".
-      case_decide as Hstate2; first subst.
+      wp_bind (Match _ _ _ _).
+      wp_apply (wp_wand (λ res,
+        ⌜res = default (fun: <> => #false)%V task⌝
+      )%I) as (res) "->".
+      { destruct task; iSteps. }
 
-      + iDestruct "Hinv_state1" as "(:inv_state_finished which=1 =2 >) /=".
-        iDestruct "Hinv_successors1" as "(:inv_successors_finished which=1 =2)".
+      wp_smart_apply (mpmc_stack_2_create_spec with "[//]") as (succs) "(#Hsuccessors_inv & Hsuccessors_model)".
+      wp_block t as "Hmeta" "(Ht_task & Ht_preds & Ht_succs & _)".
+      iMod (pointsto_persist with "Ht_succs") as "#Ht_succs".
+
+      iMod state_alloc as "(%γ_state & Hstate₁ & Hstate₂)".
+      iMod dependencies_alloc as "(%gen & Hdependencies_auth)".
+      iMod (generation_alloc gen) as "(%γ_generation & Hgeneration₁ & Hgeneration₂)".
+      iMod predecessors_alloc as "(%γ_predecessors & Hpredecessors_auth)".
+      iMod (output_alloc P) as "(%γ_output & Houtput_auth & Houtput_frag)".
+
+      pose γ := {|
+        vertex_name_successors := succs ;
+        vertex_name_state := γ_state ;
+        vertex_name_generation := γ_generation ;
+        vertex_name_predecessors := γ_predecessors ;
+        vertex_name_output := γ_output ;
+      |}.
+
+      iApply ("HΦ" $! t γ).
+      iFrame.
+      rewrite vertex_inv_unfold. iStep 2.
+      iApply inv_alloc.
+      iExists 1, Init, gen, ∅. iFrame. iSplitR "Hsuccessors_model".
+      - rewrite /inv_state /inv_state_init.
+        iExists ∅. rewrite big_sepMS_empty left_id. iSteps.
+      - iExists []. iSteps.
+    Qed.
+
+    Lemma vertex_task_spec t γ task gen :
+      {{{
+        vertex_model t γ task gen
+      }}}
+        vertex_task #t
+      {{{
+        RET task;
+        vertex_model t γ task gen
+      }}}.
+    Proof.
+      iSteps.
+    Qed.
+
+    Lemma vertex_set_task_spec t γ task1 gen task2 :
+      {{{
+        vertex_model t γ task1 gen
+      }}}
+        vertex_set_task #t task2
+      {{{
+        RET ();
+        vertex_model t γ task2 gen
+      }}}.
+    Proof.
+      iSteps.
+    Qed.
+
+    Lemma vertex_set_task'_spec t γ task1 gen task2 :
+      {{{
+        vertex_model t γ task1 gen
+      }}}
+        vertex_set_task' #t task2
+      {{{
+        RET ();
+        vertex_model t γ (fun: "ctx" => task2 "ctx" ;; #false) gen
+      }}}.
+    Proof.
+      iIntros "%Φ Hmodel HΦ".
+
+      wp_rec.
+      wp_smart_apply (vertex_set_task_spec with "Hmodel HΦ").
+    Qed.
+
+    Lemma vertex_precede_spec t1 γ1 P1 R1 t2 γ2 P2 R2 task gen :
+      {{{
+        vertex_inv t1 γ1 P1 R1 ∗
+        vertex_inv t2 γ2 P2 R2 ∗
+        vertex_model t2 γ2 task gen
+      }}}
+        vertex_precede #t1 #t2
+      {{{
+        RET ();
+        vertex_model t2 γ2 task gen ∗
+        vertex_predecessor γ1 gen
+      }}}.
+    Proof.
+      setoid_rewrite vertex_inv_unfold.
+      iIntros "%Φ ((:inv_pre =1) & (:inv_pre =2) & (:model which=2)) HΦ".
+
+      wp_rec.
+      iApply (wp_frame_wand with "[Ht2_task HΦ]"); first iAccu.
+      wp_load.
+
+      awp_smart_apply (mpmc_stack_2_is_closed_spec with "Hsuccessors1_inv") without "Hstate2₁ Hgeneration2₁".
+      iInv "Hinv_1" as "(:inv_inner which=1 =1)".
+      case_decide as Hstate1; first subst.
+
+      - iDestruct "Hinv_state1" as "(:inv_state_finished which=1 =1 >) /=".
+        iDestruct "Hinv_successors1" as "(:inv_successors_finished which=1 =1)".
         iAaccIntro with "Hsuccessors1_model"; iIntros "Hsuccs1_model !>".
         { iFrameSteps. }
-        iSplitR "Hpredecessors2_elem". { iFrameSteps. }
+        iSplitL. { iFrameSteps. }
+        iIntros "{%} _ (Hstate2₁ & Hgeneration2₁)".
+
+        iApply fupd_wp.
+        iInv "Hinv_2" as "(:inv_inner which=2 =1)".
+        iDestruct (state_agree with "Hstate2₁ Hstate2₂") as %<-.
+        iDestruct (generation_agree with "Hgeneration2₁ Hgeneration2₂") as %<-.
+        iDestruct "Hinv_state2" as "(:inv_state_init which=2 =1 >)".
+        iMod (dependencies_add γ1 with "Hdependencies2_auth") as "(Hdependencies2_auth & #Hdependencies2_elem)".
+        iDestruct (big_sepMS_insert_2 γ1 with "HΔ Hstate1₁") as "HΔ".
+        iSplitR "Hstate2₁ Hgeneration2₁".
+        { assert ({[+γ1+]} ⊎ (Δ ⊎ Π) = ({[+γ1+]} ⊎ Δ) ⊎ Π) as ->.
+          { rewrite assoc //. }
+          iFrame. rewrite /inv_state. iFrameSteps.
+        }
+        iSteps.
+
+      - iDestruct "Hinv_successors1" as "(:inv_successors which=1 =1)".
+        iAaccIntro with "Hsuccessors1_model"; iIntros "Hsuccs_model !>".
+        { iFrameSteps. rewrite bool_decide_eq_false_2 //. iSteps. }
+        iSplitL.
+        { iFrameSteps. rewrite bool_decide_eq_false_2 //. iSteps. }
         iIntros "{%} _ (Hstate2₁ & Hgeneration2₁)".
 
         wp_pures.
 
         wp_bind (FAA _ _).
-        iInv "Hinv_2" as "(:inv_inner which=2 =2)".
+        iInv "Hinv_2" as "(:inv_inner which=2 =1)".
         wp_faa.
         iDestruct (state_agree with "Hstate2₁ Hstate2₂") as %<-.
         iDestruct (generation_agree with "Hgeneration2₁ Hgeneration2₂") as %<-.
-        iDestruct "Hinv_state2" as "(:inv_state_init which=2 =2)".
-        iDestruct (predecessors_elem_of with "Hpredecessors2_auth Hpredecessors2_elem") as %Hγ1.
-        iMod (predecessors_remove with "Hpredecessors2_auth Hpredecessors2_elem") as "Hpredecessors2_auth".
-        iDestruct (big_sepMS_insert_2 γ1 with "HΔ Hstate1₁") as "HΔ".
-        iSplitR "Hstate2₁ Hgeneration2₁".
-        { replace (Δ ⊎ Π) with ({[+γ1+]} ⊎ Δ ⊎ Π ∖ {[+γ1+]}) by multiset_solver.
+        iDestruct "Hinv_state2" as "(:inv_state_init which=2 =1)".
+        iMod (dependencies_add γ1 with "Hdependencies2_auth") as "(Hdependencies2_auth & #Hdependencies2_elem)".
+        iMod (predecessors_add γ1 with "Hpredecessors2_auth") as "(Hpredecessors2_auth & Hpredecessors2_elem )".
+        iSplitR "Hstate2₁ Hgeneration2₁ Hpredecessors2_elem".
+        { assert ({[+γ1+]} ⊎ (Δ ⊎ Π) = Δ ⊎ ({[+γ1+]} ⊎ Π)) as ->.
+          { rewrite assoc (comm _ _ Δ) -assoc //. }
           iFrameSteps. iPureIntro.
-          rewrite gmultiset_size_difference; first multiset_solver.
-          rewrite gmultiset_size_singleton.
-          apply gmultiset_elem_of_size_non_empty in Hγ1.
-          lia.
+          rewrite gmultiset_size_disj_union gmultiset_size_singleton. lia.
         }
-        iSteps.
+        iIntros "!> {%}".
 
-      + iDestruct "Hinv_successors1" as "(:inv_successors which=1 =2)".
-        iAaccIntro with "Hsuccessors1_model"; iIntros "Hsuccs_model !>".
-        { iFrameSteps. rewrite bool_decide_eq_false_2 //. iSteps. }
-        iSplitL.
-        { iFrameSteps. rewrite bool_decide_eq_false_2 //. iSteps.
-          iExists (t2 :: succs). iSteps.
-          iExists γ2, P2, R2. rewrite vertex_inv_unfold. iSteps.
+        wp_pures. clear.
+
+        awp_apply (mpmc_stack_2_push_spec with "Hsuccessors1_inv") without "Hstate2₁ Hgeneration2₁".
+        iInv "Hinv_1" as "(:inv_inner which=1 =2)".
+        case_decide as Hstate2; first subst.
+
+        + iDestruct "Hinv_state1" as "(:inv_state_finished which=1 =2 >) /=".
+          iDestruct "Hinv_successors1" as "(:inv_successors_finished which=1 =2)".
+          iAaccIntro with "Hsuccessors1_model"; iIntros "Hsuccs1_model !>".
+          { iFrameSteps. }
+          iSplitR "Hpredecessors2_elem". { iFrameSteps. }
+          iIntros "{%} _ (Hstate2₁ & Hgeneration2₁)".
+
+          wp_pures.
+
+          wp_bind (FAA _ _).
+          iInv "Hinv_2" as "(:inv_inner which=2 =2)".
+          wp_faa.
+          iDestruct (state_agree with "Hstate2₁ Hstate2₂") as %<-.
+          iDestruct (generation_agree with "Hgeneration2₁ Hgeneration2₂") as %<-.
+          iDestruct "Hinv_state2" as "(:inv_state_init which=2 =2)".
+          iDestruct (predecessors_elem_of with "Hpredecessors2_auth Hpredecessors2_elem") as %Hγ1.
+          iMod (predecessors_remove with "Hpredecessors2_auth Hpredecessors2_elem") as "Hpredecessors2_auth".
+          iDestruct (big_sepMS_insert_2 γ1 with "HΔ Hstate1₁") as "HΔ".
+          iSplitR "Hstate2₁ Hgeneration2₁".
+          { replace (Δ ⊎ Π) with ({[+γ1+]} ⊎ Δ ⊎ Π ∖ {[+γ1+]}) by multiset_solver.
+            iFrameSteps. iPureIntro.
+            rewrite gmultiset_size_difference; first multiset_solver.
+            rewrite gmultiset_size_singleton.
+            apply gmultiset_elem_of_size_non_empty in Hγ1.
+            lia.
+          }
+          iSteps.
+
+        + iDestruct "Hinv_successors1" as "(:inv_successors which=1 =2)".
+          iAaccIntro with "Hsuccessors1_model"; iIntros "Hsuccs_model !>".
+          { iFrameSteps. rewrite bool_decide_eq_false_2 //. iSteps. }
+          iSplitL.
+          { iFrameSteps. rewrite bool_decide_eq_false_2 //. iSteps.
+            iExists (t2 :: succs). iSteps.
+            iExists γ2, P2, R2. rewrite vertex_inv_unfold. iSteps.
+          }
+          iSteps.
+    Qed.
+
+    #[local] Lemma vertex_release_run_spec :
+      ⊢ (
+        ∀ pool ctx t γ P R task gen,
+        {{{
+          pool_context pool ctx ∗
+          vertex_inv t γ P R ∗
+          vertex_model t γ task gen ∗
+          vertex_wp t γ P R task gen
+        }}}
+          vertex_release ctx #t
+        {{{
+          RET ();
+          pool_context pool ctx
+        }}}
+      ) ∧ (
+        ∀ pool ctx t γ P R π,
+        {{{
+          pool_context pool ctx ∗
+          vertex_inv t γ P R ∗
+          predecessors_elem γ π ∗
+          vertex_finished π
+        }}}
+          vertex_release ctx #t
+        {{{
+          RET ();
+          pool_context pool ctx
+        }}}
+      ) ∧ (
+        ∀ pool ctx t γ gen P R task,
+        {{{
+          pool_context pool ctx ∗
+          vertex_inv t γ P R ∗
+          vertex_running gen ∗
+          model' t γ task Running gen ∗
+          vertex_wp t γ P R task gen
+        }}}
+          vertex_run ctx #t
+        {{{
+          RET ();
+          pool_context pool ctx
+        }}}
+      ).
+    Proof.
+      iLöb as "HLöb".
+      iDestruct "HLöb" as "(IHrelease & IHrelease_successor & IHrun)".
+      repeat iSplit.
+
+      { iClear "IHrelease IHrelease_successor".
+        setoid_rewrite vertex_inv_unfold.
+        iIntros "%pool %ctx %t %γ %P %R %task %gen !> %Φ (Hctx & (:inv_pre) & (:model) & Htask) HΦ".
+
+        wp_rec.
+        iApply (wp_frame_wand with "HΦ").
+        wp_pures.
+
+        wp_bind (FAA _ _).
+        iInv "Hinv" as "(:inv_inner =1)".
+        wp_faa.
+        iDestruct (state_agree with "Hstate₁ Hstate₂") as %<-.
+        iDestruct (generation_agree with "Hgeneration₁ Hgeneration₂") as %<-.
+        iDestruct "Hinv_state" as "(:inv_state_init =1)".
+
+        destruct_decide (size Π = 0) as ->%gmultiset_size_empty_inv | HΠ.
+
+        - rewrite gmultiset_size_empty right_id.
+          iMod (state_update Running with "Hstate₁ Hstate₂") as "(Hstate₁ & Hstate₂)".
+          iMod (dependencies_discard with "Hdependencies_auth") as "#Hdependencies_auth".
+          iDestruct "HΔ" as "#HΔ".
+          iSplitR "Hctx Ht_task Hstate₁ Hgeneration₁ Htask". { iFrameSteps. }
+          iIntros "{%} !>".
+
+          wp_smart_apply ("IHrun" with "[$]").
+          iSteps.
+
+        - iMod (state_update Released with "Hstate₁ Hstate₂") as "(Hstate₁ & Hstate₂)".
+          iMod (dependencies_discard with "Hdependencies_auth") as "#Hdependencies_auth".
+          iSplitR "Hctx". { iFrameSteps. }
+          iSteps.
+      }
+
+      { iClear "IHrelease IHrelease_successor".
+        setoid_rewrite vertex_inv_unfold.
+        iIntros "%pool %ctx %t %γ %P %R %π !> %Φ (Hctx & (:inv_pre) & Hpredecessors_elem & #Hπ) HΦ".
+
+        wp_rec.
+        iApply (wp_frame_wand with "HΦ").
+        wp_pures.
+
+        wp_bind (FAA _ _).
+        iInv "Hinv" as "(:inv_inner)".
+        wp_faa.
+        iDestruct (predecessors_elem_of with "Hpredecessors_auth Hpredecessors_elem") as %Hπ.
+        iMod (predecessors_remove with "Hpredecessors_auth Hpredecessors_elem") as "Hpredecessors_auth".
+
+        destruct state.
+
+        - iDestruct "Hinv_state" as "(:inv_state_init)".
+          iDestruct (big_sepMS_insert_2 with "HΔ Hπ") as "HΔ".
+          apply gmultiset_elem_of_size_non_empty in Hπ as ?.
+          iSplitR "Hctx".
+          { replace (Δ ⊎ Π) with (({[+π+]} ⊎ Δ) ⊎ (Π ∖ {[+π+]})) by multiset_solver.
+            iFrameSteps. iPureIntro.
+            rewrite gmultiset_size_difference; first multiset_solver.
+            rewrite gmultiset_size_singleton.
+            lia.
+          }
+          iSteps.
+
+        - iDestruct "Hinv_state" as "(:inv_state_released)".
+          iDestruct (big_sepMS_insert_2 with "HΔ Hπ") as "-##HΔ".
+          iEval (rewrite (comm (⊎))) in "HΔ".
+          destruct_decide (size Π = 1) as HΠ.
+
+          + rewrite HΠ.
+            assert (Π = {[+π+]}) as ->.
+            { apply gmultiset_size_1_elem_of in HΠ as (π_ & ->).
+              set_solver.
+            }
+            rewrite gmultiset_difference_diag.
+
+            iMod (state_update Running with "Hstate₁ Hstate₂") as "(Hstate₁ & Hstate₂)".
+            iSplitR "Hctx Hdependencies_auth Ht_task Hstate₁ Hgeneration₁ Htask". { iFrameSteps. }
+            iIntros "{%} !>".
+
+            wp_smart_apply ("IHrun" with "[$]").
+            iSteps.
+
+          + apply gmultiset_elem_of_size_non_empty in Hπ as ?.
+            iSplitR "Hctx".
+            { replace (Δ ⊎ Π) with ((Δ ⊎ {[+π+]}) ⊎ (Π ∖ {[+π+]})) by multiset_solver.
+              iFrameSteps. iPureIntro.
+              rewrite gmultiset_size_difference; first multiset_solver.
+              rewrite gmultiset_size_singleton.
+              lia.
+            }
+            iSteps.
+
+        - iDestruct "Hinv_state" as "(:inv_state_running)".
+          exfalso. set_solver.
+
+        - iDestruct "Hinv_state" as "(:inv_state_finished)".
+          assert (Π ≠ ∅) as ?%gmultiset_size_non_empty_iff by multiset_solver.
+          iSplitR "Hctx".
+          { iFrameSteps. iPureIntro.
+            rewrite gmultiset_size_difference; first multiset_solver.
+            rewrite gmultiset_size_singleton.
+            lia.
+          }
+          iSteps.
+      }
+
+      { iClear "IHrun".
+        setoid_rewrite vertex_inv_unfold.
+        iIntros "%pool %ctx %t %γ %gen %P %R %task !> %Φ (Hctx & (:inv_pre) & #Hrunning & (:model') & Htask) HΦ".
+
+        wp_rec.
+        wp_smart_apply (pool_async_silent_spec with "[-HΦ $Hctx] HΦ"). iIntros "{%} %ctx Hctx".
+        wp_pures.
+
+        wp_bind (_ <-{preds} _)%E.
+        iInv "Hinv" as "(:inv_inner =1)".
+        wp_store.
+        iDestruct (state_agree with "Hstate₁ Hstate₂") as %<-.
+        iMod (state_update Init with "Hstate₁ Hstate₂") as "(Hstate₁ & Hstate₂)".
+        iDestruct "Hinv_state" as "(:inv_state_running =1)".
+        iMod dependencies_alloc as "(%gen' & Hdependencies_auth)".
+        iMod (generation_update gen' with "Hgeneration₁ Hgeneration₂") as "(Hgeneration₁ & Hgeneration₂)".
+        iSplitR "Hctx Ht_task Hstate₁ Hgeneration₁ Htask".
+        { iFrameSteps.
+          iExists ∅. rewrite left_id big_sepMS_empty. iSteps.
         }
-        iSteps.
-  Qed.
+        iIntros "{%} !>".
 
-  #[local] Lemma vertex_release_run_spec :
-    ⊢ (
-      ∀ pool ctx t γ P R task gen,
+        wp_load.
+
+        rewrite vertex_wp_unfold.
+        wp_apply (wp_wand with "(Htask Hctx [$] [$])") as (res) "{%} (%b & %task & -> & Hctx & (:model) & Hb)".
+        destruct b.
+
+        - wp_smart_apply ("IHrelease" with "[$]").
+          iSteps.
+
+        - iDestruct "Hb" as "(HP & #HR)".
+
+          wp_load.
+
+          awp_apply (mpmc_stack_2_close_spec with "Hsuccessors_inv") without "Hctx".
+          iInv "Hinv" as "(:inv_inner =2)".
+          iDestruct (state_agree with "Hstate₁ Hstate₂") as %<-.
+          iDestruct "Hinv_state" as "(:inv_state_init =2 >)".
+          iDestruct "Hinv_successors" as "(:inv_successors =2)".
+          iAaccIntro with "Hsuccessors_model"; iIntros "Hsuccessors_model"; first iFrameSteps.
+          iMod (state_update Finished with "Hstate₁ Hstate₂") as "(Hstate₁ & Hstate₂)".
+          iMod (state₁_discard with "Hstate₁") as "#Hstate₁".
+          iDestruct (output_produce with "Houtput_auth HP") as "Houtput_auth".
+          iSplitR "Hsuccs". { iFrameSteps. }
+          iIntros "!> H£ Hctx {%}".
+
+          iMod (lc_fupd_elim_later with "H£ Hsuccs") as "Hsuccs".
+          wp_smart_apply (clst_iter_spec (λ _, pool_context pool ctx) with "[$Hctx Hsuccs]"); [done | | iSteps].
+          rewrite big_sepL_fmap.
+          iApply (big_sepL_impl with "Hsuccs"). iIntros "!> %i %succ _ (:inv_successor) Hctx".
+          wp_smart_apply ("IHrelease_successor" with "[$Hctx $Hpredecessors_elem $Hstate₁]"); last iSteps.
+          iApply (vertex_inv_unfold with "Hinv_succ").
+      }
+    Qed.
+    Lemma vertex_release_spec pool ctx t γ P R task gen :
       {{{
         pool_context pool ctx ∗
         vertex_inv t γ P R ∗
@@ -952,220 +1158,495 @@ Section vertex_G.
       {{{
         RET ();
         pool_context pool ctx
-      }}}
-    ) ∧ (
-      ∀ pool ctx t γ P R π,
+      }}}.
+    Proof.
+      iDestruct vertex_release_run_spec as "(H & _)".
+      iApply "H".
+    Qed.
+    Lemma vertex_release_spec' pool ctx t γ P R task gen :
       {{{
         pool_context pool ctx ∗
         vertex_inv t γ P R ∗
-        predecessors_elem γ π ∗
-        vertex_finished π
+        vertex_model t γ task gen ∗
+        ( ∀ pool ctx,
+          pool_context pool ctx -∗
+          vertex_running gen -∗
+          WP task ctx {{ res,
+            ⌜res = #false⌝ ∗
+            ▷ pool_context pool ctx ∗
+            ▷ P ∗
+            ▷ □ R
+          }}
+        )
       }}}
         vertex_release ctx #t
       {{{
         RET ();
         pool_context pool ctx
-      }}}
-    ) ∧ (
-      ∀ pool ctx t γ gen P R task,
-      {{{
-        pool_context pool ctx ∗
-        vertex_inv t γ P R ∗
-        vertex_running gen ∗
-        model' t γ task Running gen ∗
-        vertex_wp t γ P R task gen
-      }}}
-        vertex_run ctx #t
-      {{{
-        RET ();
-        pool_context pool ctx
-      }}}
-    ).
+      }}}.
+    Proof.
+      iIntros "%Φ (Hctx & #Hinv & Hmodel & Htask) HΦ".
+
+      wp_apply (vertex_release_spec with "[- HΦ] HΦ").
+      rewrite vertex_wp_unfold. iFrameSteps.
+    Qed.
+  End vertex_G.
+
+  #[global] Opaque vertex_inv.
+  #[global] Opaque vertex_model.
+  #[global] Opaque vertex_output.
+  #[global] Opaque vertex_running.
+  #[global] Opaque vertex_finished.
+  #[global] Opaque vertex_predecessor.
+  #[global] Opaque vertex_wp.
+End raw.
+
+From zoo_parabs Require
+  vertex__opaque.
+
+Section vertex_G.
+  Context `{vertex_G : VertexG Σ}.
+
+  Implicit Types b : bool.
+  Implicit Types l : location.
+  Implicit Types v t task ctx : val.
+
+  Definition vertex_inv t P R : iProp Σ :=
+    ∃ l γ,
+    ⌜t = #l⌝ ∗
+    meta l nroot γ ∗
+    raw.vertex_inv l γ P R.
+  #[local] Instance : CustomIpatFormat "inv" :=
+    "(
+      %l{}{_{!}} &
+      %γ{}{_{!}} &
+      {%Heq{};->} &
+      #Hmeta{_{}}{_{!}} &
+      #Hinv{_{}}
+    )".
+
+  #[global] Instance vertex_inv_ne t n :
+    Proper (
+      (≡{n}≡) ==>
+      (≡{n}≡) ==>
+      (≡{n}≡)
+    ) (vertex_inv t).
   Proof.
-    iLöb as "HLöb".
-    iDestruct "HLöb" as "(IHrelease & IHrelease_successor & IHrun)".
-    repeat iSplit.
-
-    { iClear "IHrelease IHrelease_successor".
-      setoid_rewrite vertex_inv_unfold.
-      iIntros "%pool %ctx %t %γ %P %R %task %gen !> %Φ (Hctx & (:inv_pre) & (:model) & Htask) HΦ".
-
-      wp_rec.
-      iApply (wp_frame_wand with "HΦ").
-      wp_pures.
-
-      wp_bind (FAA _ _).
-      iInv "Hinv" as "(:inv_inner =1)".
-      wp_faa.
-      iDestruct (state_agree with "Hstate₁ Hstate₂") as %<-.
-      iDestruct (generation_agree with "Hgeneration₁ Hgeneration₂") as %<-.
-      iDestruct "Hinv_state" as "(:inv_state_init =1)".
-
-      destruct_decide (size Π = 0) as ->%gmultiset_size_empty_inv | HΠ.
-
-      - rewrite gmultiset_size_empty right_id.
-        iMod (state_update Running with "Hstate₁ Hstate₂") as "(Hstate₁ & Hstate₂)".
-        iMod (dependencies_discard with "Hdependencies_auth") as "#Hdependencies_auth".
-        iDestruct "HΔ" as "#HΔ".
-        iSplitR "Hctx Ht_task Hstate₁ Hgeneration₁ Htask". { iFrameSteps. }
-        iIntros "{%} !>".
-
-        wp_smart_apply ("IHrun" with "[$]").
-        iSteps.
-
-      - iMod (state_update Released with "Hstate₁ Hstate₂") as "(Hstate₁ & Hstate₂)".
-        iMod (dependencies_discard with "Hdependencies_auth") as "#Hdependencies_auth".
-        iSplitR "Hctx". { iFrameSteps. }
-        iSteps.
-    }
-
-    { iClear "IHrelease IHrelease_successor".
-      setoid_rewrite vertex_inv_unfold.
-      iIntros "%pool %ctx %t %γ %P %R %π !> %Φ (Hctx & (:inv_pre) & Hpredecessors_elem & #Hπ) HΦ".
-
-      wp_rec.
-      iApply (wp_frame_wand with "HΦ").
-      wp_pures.
-
-      wp_bind (FAA _ _).
-      iInv "Hinv" as "(:inv_inner)".
-      wp_faa.
-      iDestruct (predecessors_elem_of with "Hpredecessors_auth Hpredecessors_elem") as %Hπ.
-      iMod (predecessors_remove with "Hpredecessors_auth Hpredecessors_elem") as "Hpredecessors_auth".
-
-      destruct state.
-
-      - iDestruct "Hinv_state" as "(:inv_state_init)".
-        iDestruct (big_sepMS_insert_2 with "HΔ Hπ") as "HΔ".
-        apply gmultiset_elem_of_size_non_empty in Hπ as ?.
-        iSplitR "Hctx".
-        { replace (Δ ⊎ Π) with (({[+π+]} ⊎ Δ) ⊎ (Π ∖ {[+π+]})) by multiset_solver.
-          iFrameSteps. iPureIntro.
-          rewrite gmultiset_size_difference; first multiset_solver.
-          rewrite gmultiset_size_singleton.
-          lia.
-        }
-        iSteps.
-
-      - iDestruct "Hinv_state" as "(:inv_state_released)".
-        iDestruct (big_sepMS_insert_2 with "HΔ Hπ") as "-##HΔ".
-        iEval (rewrite (comm (⊎))) in "HΔ".
-        destruct_decide (size Π = 1) as HΠ.
-
-        + rewrite HΠ.
-          assert (Π = {[+π+]}) as ->.
-          { apply gmultiset_size_1_elem_of in HΠ as (π_ & ->).
-            set_solver.
-          }
-          rewrite gmultiset_difference_diag.
-
-          iMod (state_update Running with "Hstate₁ Hstate₂") as "(Hstate₁ & Hstate₂)".
-          iSplitR "Hctx Hdependencies_auth Ht_task Hstate₁ Hgeneration₁ Htask". { iFrameSteps. }
-          iIntros "{%} !>".
-
-          wp_smart_apply ("IHrun" with "[$]").
-          iSteps.
-
-        + apply gmultiset_elem_of_size_non_empty in Hπ as ?.
-          iSplitR "Hctx".
-          { replace (Δ ⊎ Π) with ((Δ ⊎ {[+π+]}) ⊎ (Π ∖ {[+π+]})) by multiset_solver.
-            iFrameSteps. iPureIntro.
-            rewrite gmultiset_size_difference; first multiset_solver.
-            rewrite gmultiset_size_singleton.
-            lia.
-          }
-          iSteps.
-
-      - iDestruct "Hinv_state" as "(:inv_state_running)".
-        exfalso. set_solver.
-
-      - iDestruct "Hinv_state" as "(:inv_state_finished)".
-        assert (Π ≠ ∅) as ?%gmultiset_size_non_empty_iff by multiset_solver.
-        iSplitR "Hctx".
-        { iFrameSteps. iPureIntro.
-          rewrite gmultiset_size_difference; first multiset_solver.
-          rewrite gmultiset_size_singleton.
-          lia.
-        }
-        iSteps.
-    }
-
-    { iClear "IHrun".
-      setoid_rewrite vertex_inv_unfold.
-      iIntros "%pool %ctx %t %γ %gen %P %R %task !> %Φ (Hctx & (:inv_pre) & #Hrunning & (:model') & Htask) HΦ".
-
-      wp_rec.
-      wp_smart_apply (pool_async_silent_spec with "[-HΦ $Hctx] HΦ"). iIntros "{%} %ctx Hctx".
-      wp_pures.
-
-      wp_bind (_ <-{preds} _)%E.
-      iInv "Hinv" as "(:inv_inner =1)".
-      wp_store.
-      iDestruct (state_agree with "Hstate₁ Hstate₂") as %<-.
-      iMod (state_update Init with "Hstate₁ Hstate₂") as "(Hstate₁ & Hstate₂)".
-      iDestruct "Hinv_state" as "(:inv_state_running =1)".
-      iMod dependencies_alloc as "(%gen' & Hdependencies_auth)".
-      iMod (generation_update gen' with "Hgeneration₁ Hgeneration₂") as "(Hgeneration₁ & Hgeneration₂)".
-      iSplitR "Hctx Ht_task Hstate₁ Hgeneration₁ Htask".
-      { iFrameSteps.
-        iExists ∅. rewrite left_id big_sepMS_empty. iSteps.
-      }
-      iIntros "{%} !>".
-
-      wp_load.
-
-      rewrite vertex_wp_unfold.
-      wp_apply (wp_wand with "(Htask Hctx [$] [$])") as (res) "{%} (%b & %task & -> & Hctx & (:model) & Hb)".
-      destruct b.
-
-      - wp_smart_apply ("IHrelease" with "[$]").
-        iSteps.
-
-      - iDestruct "Hb" as "(HP & #HR)".
-
-        wp_load.
-
-        awp_apply (mpmc_stack_2_close_spec with "Hsuccessors_inv") without "Hctx".
-        iInv "Hinv" as "(:inv_inner =2)".
-        iDestruct (state_agree with "Hstate₁ Hstate₂") as %<-.
-        iDestruct "Hinv_state" as "(:inv_state_init =2 >)".
-        iDestruct "Hinv_successors" as "(:inv_successors =2)".
-        iAaccIntro with "Hsuccessors_model"; iIntros "Hsuccessors_model"; first iFrameSteps.
-        iMod (state_update Finished with "Hstate₁ Hstate₂") as "(Hstate₁ & Hstate₂)".
-        iMod (state₁_discard with "Hstate₁") as "#Hstate₁".
-        iDestruct (output_produce with "Houtput_auth HP") as "Houtput_auth".
-        iSplitR "Hsuccs". { iFrameSteps. }
-        iIntros "!> H£ Hctx {%}".
-
-        iMod (lc_fupd_elim_later with "H£ Hsuccs") as "Hsuccs".
-        wp_smart_apply (clst_iter_spec (λ _, pool_context pool ctx) with "[$Hctx Hsuccs]"); [done | | iSteps].
-        rewrite big_sepL_fmap.
-        iApply (big_sepL_impl with "Hsuccs"). iIntros "!> %i %succ _ (:inv_successor) Hctx".
-        wp_smart_apply ("IHrelease_successor" with "[$Hctx $Hpredecessors_elem $Hstate₁]"); last iSteps.
-        iApply (vertex_inv_unfold with "Hinv_succ").
-    }
+    solve_proper.
   Qed.
-  Lemma vertex_release_spec pool ctx t γ P R task gen :
+  #[global] Instance vertex_inv_proper t :
+    Proper (
+      (≡) ==>
+      (≡) ==>
+      (≡)
+    ) (vertex_inv t).
+  Proof.
+    solve_proper.
+  Qed.
+
+  Definition vertex_model t task gen : iProp Σ :=
+    ∃ l γ,
+    ⌜t = #l⌝ ∗
+    meta l nroot γ ∗
+    raw.vertex_model l γ task gen.
+  #[local] Instance : CustomIpatFormat "model" :=
+    "(
+      %l{}{_{!}} &
+      %γ{}{_{!}} &
+      {%Heq{};->} &
+      #Hmeta{_{}}{_{!}} &
+      Hmodel{_{}}
+    )".
+
+  Definition vertex_output t Q : iProp Σ :=
+    ∃ l γ,
+    ⌜t = #l⌝ ∗
+    meta l nroot γ ∗
+    raw.vertex_output γ Q.
+  #[local] Instance : CustomIpatFormat "output" :=
+    "(
+      %l{}{_{!}} &
+      %γ{}{_{!}} &
+      {%Heq{};->} &
+      #Hmeta{_{}}{_{!}} &
+      Houtput{_{}}
+    )".
+
+  Definition vertex_running :=
+    raw.vertex_running.
+
+  Definition vertex_finished t : iProp Σ :=
+    ∃ l γ,
+    ⌜t = #l⌝ ∗
+    meta l nroot γ ∗
+    raw.vertex_finished γ.
+  #[local] Instance : CustomIpatFormat "finished" :=
+    "(
+      %l{}{_{!}} &
+      %γ{}{_{!}} &
+      {%Heq{};->} &
+      #Hmeta{_{}}{_{!}} &
+      Hfinished{_{}}
+    )".
+
+  Definition vertex_predecessor t gen : iProp Σ :=
+    ∃ l γ,
+    ⌜t = #l⌝ ∗
+    meta l nroot γ ∗
+    raw.vertex_predecessor γ gen.
+  #[local] Instance : CustomIpatFormat "predecessor" :=
+    "(
+      %l{}{_{!}} &
+      %γ{}{_{!}} &
+      {%Heq{};->} &
+      #Hmeta{_{}}{_{!}} &
+      Hpredecessor{_{}}
+    )".
+
+  Definition vertex_wp_body t P R body task gen : iProp Σ :=
+    ∀ pool ctx gen',
+    pool_context pool ctx -∗
+    vertex_running gen -∗
+    vertex_model t task gen' -∗
+    WP task ctx {{ res,
+      ∃ b task,
+      ⌜res = #b⌝ ∗
+      ▷ (
+        pool_context pool ctx ∗
+        vertex_model t task gen' ∗
+        if b then
+          body task gen'
+        else
+          P ∗
+          □ R
+      )
+    }}.
+  #[local] Definition vertex_wp_pre
+  : val → iProp Σ → iProp Σ →
+    (val -d> vertex_generation -d> iProp Σ) →
+    val -d> vertex_generation -d> iProp Σ
+  :=
+    vertex_wp_body.
+  #[local] Instance vertex_wp_pre_contractive t P R :
+    Contractive (vertex_wp_pre t P R).
+  Proof.
+    rewrite /vertex_wp_pre /vertex_wp_body.
+    solve_contractive.
+  Qed.
+  #[local] Instance vertex_wp_pre_ne t P R :
+    NonExpansive (vertex_wp_pre t P R).
+  Proof.
+    apply _.
+  Qed.
+  Definition vertex_wp t P R : val → vertex_generation → iProp Σ :=
+    fixpoint (vertex_wp_pre t P R).
+
+  Lemma vertex_wp_unfold t P R task gen :
+    vertex_wp t P R task gen ⊣⊢
+    vertex_wp_body t P R (vertex_wp t P R) task gen.
+  Proof.
+    apply (fixpoint_unfold (vertex_wp_pre t P R)).
+  Qed.
+  #[global] Instance vertex_wp_ne n :
+    Proper (
+      (=) ==>
+      (≡{n}≡) ==>
+      (≡{n}≡) ==>
+      (≡{n}≡) ==>
+      (≡{n}≡) ==>
+      (≡{n}≡)
+    ) vertex_wp.
+  Proof.
+    intros t t_ <-.
+    induction (lt_wf n) as [n _ IH] => P1 P2 HP R1 R2 HR task task_ <- gen gen_ <-.
+    rewrite !vertex_wp_unfold /vertex_wp_body.
+    do 16 f_equiv. f_contractive.
+    apply (dist_le _ m) in HP; last by apply SIdx.lt_le_incl.
+    apply (dist_le _ m) in HR; last by apply SIdx.lt_le_incl.
+    do 3 f_equiv; last solve_proper.
+    apply IH; done.
+  Qed.
+  #[local] Lemma vertex_wp_to_raw l γ P R task gen :
+    meta l nroot γ -∗
+    vertex_wp #l P R task gen -∗
+    raw.vertex_wp l γ P R task gen.
+  Proof.
+    iLöb as "HLöb" forall (task gen).
+
+    iEval (rewrite vertex_wp_unfold raw.vertex_wp_unfold).
+    iIntros "#Hmeta Hwp %pool %ctx %gen' Hctx Hrunning Hmodel".
+
+    wp_apply (wp_wand with "(Hwp Hctx Hrunning [$Hmodel])") as (res) "{%} (%b & %task & -> & ($ & Hmodel & Hwp))"; first iSteps.
+    iExists b, task. iStep. iModIntro.
+    iDestruct "Hmodel" as "(:model =1)". simplify.
+    iDestruct (meta_agree with "Hmeta Hmeta_1") as %<-. iClear "Hmeta_1".
+    destruct b; iFrameSteps.
+  Qed.
+
+  #[global] Instance vertex_output_contractive t :
+    Contractive (vertex_output t).
+  Proof.
+    solve_contractive.
+  Qed.
+  #[global] Instance vertex_output_proper t :
+    Proper ((≡) ==> (≡)) (vertex_output t).
+  Proof.
+    solve_proper.
+  Qed.
+
+  #[global] Instance vertex_model_timeless t task gen :
+    Timeless (vertex_model t task gen).
+  Proof.
+    apply _.
+  Qed.
+  #[global] Instance vertex_running_timeless gen :
+    Timeless (vertex_running gen).
+  Proof.
+    apply _.
+  Qed.
+  #[global] Instance vertex_finished_timeless t :
+    Timeless (vertex_finished t).
+  Proof.
+    apply _.
+  Qed.
+  #[global] Instance vertex_predecessor_timeless t gen :
+    Timeless (vertex_predecessor t gen).
+  Proof.
+    apply _.
+  Qed.
+
+  #[global] Instance vertex_inv_persistent t P R :
+    Persistent (vertex_inv t P R).
+  Proof.
+    apply _.
+  Qed.
+  #[global] Instance vertex_running_persistent gen :
+    Persistent (vertex_running gen).
+  Proof.
+    apply _.
+  Qed.
+  #[global] Instance vertex_finished_persistent t :
+    Persistent (vertex_finished t).
+  Proof.
+    apply _.
+  Qed.
+  #[global] Instance vertex_predecessor_persistent t gen :
+    Persistent (vertex_predecessor t gen).
+  Proof.
+    apply _.
+  Qed.
+
+  Lemma vertex_model_exclusive t task1 gen1 task2 gen2 :
+    vertex_model t task1 gen1 -∗
+    vertex_model t task2 gen2 -∗
+    False.
+  Proof.
+    iIntros "(:model =1) (:model =2)". simplify.
+    iDestruct (meta_agree with "Hmeta_1 Hmeta_2") as %<-.
+    iApply (raw.vertex_model_exclusive with "Hmodel_1 Hmodel_2").
+  Qed.
+  Lemma vertex_model_finished t task gen :
+    vertex_model t task gen -∗
+    vertex_finished t -∗
+    False.
+  Proof.
+    iIntros "(:model =1) (:finished =2)". simplify.
+    iDestruct (meta_agree with "Hmeta_1 Hmeta_2") as %<-.
+    iApply (raw.vertex_model_finished with "Hmodel_1 Hfinished_2").
+  Qed.
+
+  Lemma vertex_output_divide {t P R Q} Qs :
+    vertex_inv t P R -∗
+    vertex_output t Q -∗
+    (Q -∗ [∗ list] Q ∈ Qs, Q) ={⊤}=∗
+    [∗ list] Q ∈ Qs, vertex_output t Q.
+  Proof.
+    iIntros "(:inv =1) (:output =2) H". simplify.
+    iDestruct (meta_agree with "Hmeta_1 Hmeta_2") as %<-.
+    iMod (raw.vertex_output_divide with "Hinv_1 Houtput_2 H") as "H".
+    iApply (big_sepL_impl with "H").
+    iSteps.
+  Qed.
+  Lemma vertex_output_split {t P R Q} Q1 Q2 :
+    vertex_inv t P R -∗
+    vertex_output t Q -∗
+    (Q -∗ Q1 ∗ Q2) ={⊤}=∗
+      vertex_output t Q1 ∗
+      vertex_output t Q2.
+  Proof.
+    iIntros "(:inv =1) (:output =2) H". simplify.
+    iDestruct (meta_agree with "Hmeta_1 Hmeta_2") as %<-.
+    iMod (raw.vertex_output_split with "Hinv_1 Houtput_2 H") as "H".
+    iSteps.
+  Qed.
+
+  Lemma vertex_predecessor_finished t gen :
+    vertex_predecessor t gen -∗
+    vertex_running gen -∗
+    vertex_finished t.
+  Proof.
+    iIntros "(:predecessor) Hrunning". simplify.
+    iDestruct (raw.vertex_predecessor_finished with "Hpredecessor Hrunning") as "Hfinished".
+    iSteps.
+  Qed.
+
+  Lemma vertex_inv_finished t P R :
+    vertex_inv t P R -∗
+    vertex_finished t ={⊤}=∗
+    ▷ □ R.
+  Proof.
+    iIntros "(:inv =1) (:finished =2)". simplify.
+    iDestruct (meta_agree with "Hmeta_1 Hmeta_2") as %<-.
+    iApply (raw.vertex_inv_finished with "Hinv_1 Hfinished_2").
+  Qed.
+  Lemma vertex_inv_finished' t P R :
+    £ 1 -∗
+    vertex_inv t P R -∗
+    vertex_finished t ={⊤}=∗
+    □ R.
+  Proof.
+    iIntros "H£ (:inv =1) (:finished =2)". simplify.
+    iDestruct (meta_agree with "Hmeta_1 Hmeta_2") as %<-.
+    iApply (raw.vertex_inv_finished' with "H£ Hinv_1 Hfinished_2").
+  Qed.
+  Lemma vertex_inv_finished_output t P R Q :
+    vertex_inv t P R -∗
+    vertex_finished t -∗
+    vertex_output t Q ={⊤}=∗
+    ▷^2 Q.
+  Proof.
+    iIntros "(:inv =1) (:finished =2) (:output =3)". simplify.
+    iDestruct (meta_agree with "Hmeta_1 Hmeta_2") as %<-.
+    iDestruct (meta_agree with "Hmeta_1 Hmeta_3") as %<-.
+    iApply (raw.vertex_inv_finished_output with "Hinv_1 Hfinished_2 Houtput_3").
+  Qed.
+  Lemma vertex_inv_finished_output' t P R Q :
+    £ 2 -∗
+    vertex_inv t P R -∗
+    vertex_finished t -∗
+    vertex_output t Q ={⊤}=∗
+    Q.
+  Proof.
+    iIntros "H£ (:inv =1) (:finished =2) (:output =3)". simplify.
+    iDestruct (meta_agree with "Hmeta_1 Hmeta_2") as %<-.
+    iDestruct (meta_agree with "Hmeta_1 Hmeta_3") as %<-.
+    iApply (raw.vertex_inv_finished_output' with "H£ Hinv_1 Hfinished_2 Houtput_3").
+  Qed.
+
+  Lemma vertex_create_spec P R (task : option val) :
+    {{{
+      True
+    }}}
+      vertex_create task
+    {{{ t gen,
+      RET t;
+      vertex_inv t P R ∗
+      vertex_model t (default (fun: <> => #false)%V task) gen ∗
+      vertex_output t P
+    }}}.
+  Proof.
+    iIntros "%Φ _ HΦ".
+
+    iApply wp_fupd.
+    wp_apply (raw.vertex_create_spec with "[//]") as (l γ gen) "(Hmeta & #Hinv & Hmodel & Houtput)".
+    iMod (meta_set with "Hmeta") as "#Hmeta"; first done.
+    iSteps.
+  Qed.
+
+  Lemma vertex_task_spec t task gen :
+    {{{
+      vertex_model t task gen
+    }}}
+      vertex_task t
+    {{{
+      RET task;
+      vertex_model t task gen
+    }}}.
+  Proof.
+    iIntros "%Φ (:model) HΦ".
+
+    wp_apply (raw.vertex_task_spec with "[$]").
+    iSteps.
+  Qed.
+
+  Lemma vertex_set_task_spec t task1 gen task2 :
+    {{{
+      vertex_model t task1 gen
+    }}}
+      vertex_set_task t task2
+    {{{
+      RET ();
+      vertex_model t task2 gen
+    }}}.
+  Proof.
+    iIntros "%Φ (:model) HΦ".
+
+    wp_apply (raw.vertex_set_task_spec with "[$]").
+    iSteps.
+  Qed.
+
+  Lemma vertex_set_task'_spec t task1 gen task2 :
+    {{{
+      vertex_model t task1 gen
+    }}}
+      vertex_set_task' t task2
+    {{{
+      RET ();
+      vertex_model t (fun: "ctx" => task2 "ctx" ;; #false) gen
+    }}}.
+  Proof.
+    iIntros "%Φ (:model) HΦ".
+
+    wp_apply (raw.vertex_set_task'_spec with "[$]").
+    iSteps.
+  Qed.
+
+  Lemma vertex_precede_spec t1 P1 R1 t2 P2 R2 task gen :
+    {{{
+      vertex_inv t1 P1 R1 ∗
+      vertex_inv t2 P2 R2 ∗
+      vertex_model t2 task gen
+    }}}
+      vertex_precede t1 t2
+    {{{
+      RET ();
+      vertex_model t2 task gen ∗
+      vertex_predecessor t1 gen
+    }}}.
+  Proof.
+    iIntros "%Φ ((:inv =1) & (:inv =2) & Hmodel_2) HΦ". simplify.
+    iDestruct "Hmodel_2" as "(:model =2 !=)". simplify.
+    iDestruct (meta_agree with "Hmeta_2 Hmeta_2_") as %<-. iClear "Hmeta_2_".
+
+    wp_apply (raw.vertex_precede_spec with "[$Hmodel_2]").
+    { iFrame "#". }
+    iSteps.
+  Qed.
+
+  Lemma vertex_release_spec pool ctx t P R task gen :
     {{{
       pool_context pool ctx ∗
-      vertex_inv t γ P R ∗
-      vertex_model t γ task gen ∗
-      vertex_wp t γ P R task gen
+      vertex_inv t P R ∗
+      vertex_model t task gen ∗
+      vertex_wp t P R task gen
     }}}
-      vertex_release ctx #t
+      vertex_release ctx t
     {{{
       RET ();
       pool_context pool ctx
     }}}.
   Proof.
-    iDestruct vertex_release_run_spec as "(H & _)".
-    iApply "H".
+    iIntros "%Φ (Hctx & (:inv =1) & (:model =2) & Hwp) HΦ". simplify.
+    iDestruct (meta_agree with "Hmeta_1 Hmeta_2") as %<-. iClear "Hmeta_2".
+    iDestruct (vertex_wp_to_raw with "Hmeta_1 Hwp") as "Hwp".
+
+    wp_apply (raw.vertex_release_spec with "[$] HΦ").
   Qed.
-  Lemma vertex_release_spec' pool ctx t γ P R task gen :
+  Lemma vertex_release_spec' pool ctx t P R task gen :
     {{{
       pool_context pool ctx ∗
-      vertex_inv t γ P R ∗
-      vertex_model t γ task gen ∗
+      vertex_inv t P R ∗
+      vertex_model t task gen ∗
       ( ∀ pool ctx,
         pool_context pool ctx -∗
         vertex_running gen -∗
@@ -1177,7 +1658,7 @@ Section vertex_G.
         }}
       )
     }}}
-      vertex_release ctx #t
+      vertex_release ctx t
     {{{
       RET ();
       pool_context pool ctx
@@ -1186,12 +1667,9 @@ Section vertex_G.
     iIntros "%Φ (Hctx & #Hinv & Hmodel & Htask) HΦ".
 
     wp_apply (vertex_release_spec with "[- HΦ] HΦ").
-    rewrite vertex_wp_unfold. iFrameSteps.
+    rewrite vertex_wp_unfold. iFrame "#∗". iSteps.
   Qed.
 End vertex_G.
-
-From zoo_parabs Require
-  vertex__opaque.
 
 #[global] Opaque vertex_inv.
 #[global] Opaque vertex_model.
